proof/invariants/DeletePartition.v
@@ -32,19 +32,1954 @@
 (*  knowledge of the CeCILL license and that you accept its terms.             *)
 (*******************************************************************************)
 
-Require Import Model.ADT Model.Lib Model.MAL.
+Require Import Model.ADT Model.Lib Model.MAL Model.Monad.
 Require Import Core.Services.
 
 Require Import Proof.Isolation Proof.Hoare Proof.Consistency Proof.WeakestPreconditions
-Proof.StateLib (*Proof.InternalLemmas*) Proof.InternalLemmas2 Proof.DependentTypeLemmas.
+Proof.StateLib (*Proof.InternalLemmas*) Proof.InternalLemmas2 Proof.DependentTypeLemmas Proof.InternalLemmas3.
 
 Require Import Invariants findBlockInKSWithAddr eraseBlock checkBlockCut writeAccessibleToAncestorsIfNotCutRec.
-Require Import deleteProps.
+Require Import deleteProps initStructure.
 
 Require Import Model.Monad.
 
 From Stdlib Require Import List Bool Lia.
 Import List.ListNotations.
+
+Definition kernInSameBlock s :=
+forall parentBlock part idx block,
+In part (getPartitions multiplexer s)
+-> In parentBlock (getMappedBlocks part s)
+-> In block (getAllPaddrAux [parentBlock] s)
+-> bentryBlockIndex block idx s
+-> In (CPaddr (block-idx)) (getAllPaddrAux [parentBlock] s).
+
+Definition blockAndSh1InSameBlock s :=
+forall (block:paddr) parentBlock,
+In (CPaddr (block+sh1offset)) (getAllPaddrAux [parentBlock] s)
+-> In block (getAllPaddrAux [parentBlock] s).
+
+Definition blockAndSceInSameBlock s :=
+forall (block:paddr) parentBlock,
+In (CPaddr (block+scoffset)) (getAllPaddrAux [parentBlock] s)
+-> In block (getAllPaddrAux [parentBlock] s).
+
+(*for now, partial consistency1. TODO add consistency2 and the isolation props*)
+Definition deleteProps s blockToDelete blockStartAddr:=
+  nullAddrExists s
+  /\ wellFormedFstShadowIfBlockEntry s
+  /\ (*partial PDTIfPDFlag*)
+      (forall idPDchild sh1entryaddr part, idPDchild <> blockToDelete
+        -> In part (getPartitions multiplexer s)
+        -> In idPDchild (getMappedBlocks part s)
+        -> true = checkChild idPDchild s sh1entryaddr /\ sh1entryAddr idPDchild sh1entryaddr s
+        -> bentryAFlag idPDchild false s /\ bentryPFlag idPDchild true s
+            /\ (exists startaddr, bentryStartAddr idPDchild startaddr s /\ entryPDT idPDchild startaddr s))
+  /\ AccessibleNoPDFlag s
+  /\ FirstFreeSlotPointerIsBEAndFreeSlot s
+  /\ multiplexerIsPDT s
+  /\ currentPartitionInPartitionsList s
+  /\ wellFormedShadowCutIfBlockEntry s
+  /\ BlocksRangeFromKernelStartIsBE s
+  /\ KernelStructureStartFromBlockEntryAddrIsKS s
+  /\ sh1InChildLocationIsBE s
+  /\ StructurePointerIsKS s
+  /\ NextKSIsKS s
+  /\ NextKSOffsetIsPADDR s
+  /\ NoDupInFreeSlotsList s
+  /\ freeSlotsListIsFreeSlot s
+  /\ DisjointFreeSlotsLists s
+  /\ inclFreeSlotsBlockEntries s
+  /\ DisjointKSEntries s
+  /\ noDupPartitionTree s
+  /\ (*partial isParent*)
+      (forall partition pdparent,
+        partition <> blockStartAddr
+        -> In pdparent (getPartitions multiplexer s)
+        -> In partition (getChildren pdparent s) -> pdentryParent partition pdparent s)
+  /\ isChild s
+  /\ noDupKSEntriesList s
+  /\ noDupMappedBlocksList s
+  /\ wellFormedBlock s
+  /\ NbFreeSlotsISNbFreeSlotsInList s
+  /\ maxNbPrepareIsMaxNbKernels s
+  /\ blockInChildHasAtLeastEquivalentBlockInParent s
+  /\ partitionTreeIsTree s
+  /\ nextKernelIsValid s
+  /\ noDupListOfKerns s
+  /\ MPUsizeIsBelowMax s
+  /\ originIsParentBlocksStart s
+  /\ nextImpliesBlockWasCut s
+  /\ blocksAddressesTypes s
+  /\ notPDTIfNotPDflag s
+  /\ nextKernAddrIsInSameBlock s
+  /\ PDflagMeansNoChild s
+  /\ nbPrepareIsNbKern s
+  /\ pdchildIsPDT s
+  /\ childBlockNullIfChildNull s
+  /\ accessibleBlocksArePresent s
+  /\ sharedBlockIsPresent s
+  /\ (*partial sharedBlockNoPDflagNoLocIsKern (modified version)*)
+      (forall part block child startaddr,
+        child <> blockStartAddr
+        -> In part (getPartitions multiplexer s)
+        -> In block (getMappedBlocks part s)
+        -> sh1entryPDchild (CPaddr (block + sh1offset)) child s
+        -> child <> nullAddr
+        -> sh1entryPDflag (CPaddr (block + sh1offset)) false s
+        -> sh1entryInChildLocationWeak (CPaddr (block + sh1offset)) nullAddr s
+        -> bentryStartAddr block startaddr s
+        -> In startaddr (getConfigBlocks child s)
+            /\ (forall addr child2, In addr (getAllPaddrAux [block] s)
+                  -> In child2 (getChildren part s)
+                  -> ~In addr (getMappedPaddr child2 s))
+            /\ (forall (addr:paddr) endaddr part2, bentryEndAddr block endaddr s
+                  -> In part2 (getPartitions multiplexer s)
+                  -> startaddr+Constants.kernelStructureTotalLength <= addr
+                  -> addr < endaddr
+                  -> ~In addr (getConfigPaddr part2 s))) (*TODO is that prop propagated ?*)
+  /\ partitionNotAutoMapped s
+  /\ configAddrNotMappedInChild s
+  /\ fullKernelIsInOneBlock s
+  /\ (*partial sharedBlocksAdressesAreAllMappedInChild*)
+      (forall partition block sh1entryaddr blockChild idchild,
+        idchild <> blockStartAddr
+        -> In partition (getPartitions multiplexer s)
+        -> In block (getMappedBlocks partition s)
+        -> sh1entryAddr block sh1entryaddr s
+        -> sh1entryPDchild sh1entryaddr idchild s
+        -> sh1entryInChildLocationWeak sh1entryaddr blockChild s
+        -> idchild <> nullAddr
+        -> blockChild <> nullAddr
+        -> forall addr, In addr (getAllPaddrAux [block] s) -> In addr (getMappedPaddr idchild s))
+  /\ kernInSameBlock s
+  /\ blockAndSh1InSameBlock s
+  /\ blockAndSceInSameBlock s.
+
+Lemma deleteSharedBlocksInStructRecAux n currentPart kernel blockTDParent blockToDelete (currIdx:index)
+(P: state->Prop):
+{{ fun s => deleteProps s blockTDParent blockToDelete /\ n > currIdx /\ currIdx < kernelStructureEntriesNb
+    /\ isKS kernel s
+    /\ lookup blockToDelete (memory s) beqAddr = None
+    /\ bentryStartAddr blockTDParent blockToDelete s
+    /\ ~In blockToDelete (getPartitions multiplexer s)
+    /\ (forall blockIdx, blockIdx < kernelStructureEntriesNb
+          -> In (CPaddr (kernel+blockIdx)) (filterOptionPaddr (getKSEntries currentPart s)))
+    /\ In currentPart (getPartitions multiplexer s)
+    /\ isPDT currentPart s
+    /\ (forall block startBlock endBlock, In block (getMappedBlocks currentPart s)
+          -> sh1entryPDchild (CPaddr (block+sh1offset)) blockToDelete s
+          -> bentryStartAddr block startBlock s
+          -> bentryEndAddr block endBlock s
+          -> (forall addr, In addr (getAllPaddrBlock startBlock endBlock)
+              -> ~In addr (getPartitions multiplexer s)
+                  /\ (forall part, In part (getPartitions multiplexer s)
+                      -> ~In addr (filterOptionPaddr (getKSEntries part s))
+                          /\ ~In addr (getConfigPaddr part s))
+                  /\ (isBE addr s -> addr + scoffset < endBlock)
+                  /\ (isKS addr s -> addr + nextoffset < endBlock)
+                  /\ addr <> nullAddr))
+}}
+Internal.deleteSharedBlocksInStructRecAux n currentPart kernel blockToDelete currIdx
+{{ fun _ s => deleteProps s blockTDParent blockToDelete
+}}.
+Proof.
+revert currIdx. induction n; simpl; intro currIdx.
+{
+  eapply weaken. apply WP.ret. intros s Hprops. exfalso. destruct Hprops as (_ & Hcontra & _). lia.
+}
+eapply bindRev.
+{ (** MAL.getBlockEntryAddrFromKernelStructureStart **)
+  eapply weaken. apply getBlockEntryAddrFromKernelStructureStartLight. intros s Hprops. apply Hprops.
+}
+intro currBlock. eapply bindRev.
+{ (** MAL.readBlockStartFromBlockEntryAddr **)
+  eapply weaken. apply readBlockStartFromBlockEntryAddr. intros s Hprops. split. apply Hprops.
+  assert(Hres: BlocksRangeFromKernelStartIsBE s) by (unfold deleteProps in *; intuition).
+  destruct Hprops as ((Hprops & _ & HltIdxKernEntriesNb & HkernIsKS & _) & HcurrBlock). cbn in HcurrBlock.
+  rewrite PeanoNat.Nat.add_0_r in HcurrBlock. subst currBlock. apply Hres; trivial.
+}
+intro startBlock. eapply bindRev.
+{ (** MAL.readBlockEndFromBlockEntryAddr **)
+  eapply weaken. apply readBlockEndFromBlockEntryAddr. intros s Hprops. split. apply Hprops.
+  assert(Hres: BlocksRangeFromKernelStartIsBE s) by (unfold deleteProps in *; intuition).
+  destruct Hprops as (_ & Hstart). unfold bentryStartAddr in *. unfold isBE.
+  destruct (lookup currBlock (memory s) beqAddr); try(congruence). destruct v; try(congruence). trivial.
+}
+intro endBlock. eapply bindRev.
+{ (** MAL.readSh1PDChildFromBlockEntryAddr **)
+  eapply weaken. apply readSh1PDChildFromBlockEntryAddr. intros s Hprops. split. apply Hprops.
+  destruct Hprops as ((((Hprops & _) & _) & _) & Hend). unfold deleteProps in *. intuition.
+  unfold bentryEndAddr in *.
+  destruct (lookup currBlock (memory s) beqAddr); try(exfalso; congruence). destruct v; try(exfalso; congruence).
+  exists b. reflexivity.
+}
+intro currPDChild. destruct (beqAddr currPDChild blockToDelete) eqn:HbeqChildBTD.
+- rewrite <-beqAddrTrue in HbeqChildBTD. subst currPDChild. eapply bindRev.
+  { (** MAL.writeBlockAccessibleFromBlockEntryAddr **)
+    eapply weaken. apply writeBlockAccessibleFromBlockEntryAddr. intros s Hprops.
+    destruct Hprops as (((((Hprops & HgtNIdx & HltIdxKernEntriesNb & HkernIsKS & HlookupBTD & HstartBTDP &
+      HBTDNotMapped & HblocksInCurr & HcurrIsPart & HcurrIsPDT & HpropsAddrToRemove) & HcurrBlock) & Hstart) & Hend) &
+      [_ [sh1entryaddr (_ & HPDchild & Hsh1)]]).
+    unfold sh1entryAddr in *.
+    destruct (lookup currBlock (memory s) beqAddr) eqn:HlookupCurr; try(exfalso; congruence).
+    destruct v; try(exfalso; congruence). exists b. split; trivial. cbn in HcurrBlock.
+    rewrite PeanoNat.Nat.add_0_r in HcurrBlock.
+    instantiate(1 := fun _ s => exists s0 bentry0 sh1entryaddr,
+      s = {|
+            currentPartition := currentPartition s0;
+            memory :=
+              add currBlock
+                (BE (CBlockEntry (read bentry0) (write bentry0) (exec bentry0) (present bentry0) true
+                  (blockindex bentry0) (blockrange bentry0)))
+                (memory s0) beqAddr
+          |}
+      /\ lookup currBlock (memory s0) beqAddr = Some (BE bentry0)
+      /\ lookup blockToDelete (memory s0) beqAddr = None
+      /\ bentryStartAddr blockTDParent blockToDelete s0
+      /\ ~In blockToDelete (getPartitions multiplexer s0)
+      /\ (forall blockIdx, blockIdx < kernelStructureEntriesNb
+            -> In (CPaddr (kernel+blockIdx)) (filterOptionPaddr (getKSEntries currentPart s0)))
+      /\ In currentPart (getPartitions multiplexer s0)
+      /\ isPDT currentPart s0
+      /\ sh1entryaddr = CPaddr (currBlock + sh1offset)
+      /\ deleteProps s0 blockTDParent blockToDelete /\ S n > currIdx /\ currIdx < kernelStructureEntriesNb
+      /\ isKS kernel s0 /\ currBlock = CPaddr (kernel + currIdx)
+      /\ bentryStartAddr currBlock startBlock s0
+      /\ bentryEndAddr currBlock endBlock s0
+      /\ sh1entryPDchild sh1entryaddr blockToDelete s0
+      /\ (forall block startBlock endBlock, In block (getMappedBlocks currentPart s0)
+          -> sh1entryPDchild (CPaddr (block+sh1offset)) blockToDelete s0
+          -> bentryStartAddr block startBlock s0
+          -> bentryEndAddr block endBlock s0
+          -> (forall addr, In addr (getAllPaddrBlock startBlock endBlock)
+              -> ~In addr (getPartitions multiplexer s0)
+                  /\ (forall part, In part (getPartitions multiplexer s0)
+                      -> ~In addr (filterOptionPaddr (getKSEntries part s0))
+                          /\ ~In addr (getConfigPaddr part s0))
+                  /\ (isBE addr s0 -> addr + scoffset < endBlock)
+                  /\ (isKS addr s0 -> addr + nextoffset < endBlock)
+                  /\ addr <> nullAddr))). exists s. exists b. exists sh1entryaddr.
+    intuition.
+  }
+  intro. eapply bindRev.
+  { (** MAL.writeSh1EntryFromBlockEntryAddrLight **)
+    eapply weaken. apply writeSh1EntryFromBlockEntryAddrLight. intros s Hprops.
+    destruct Hprops as [s0 [bentry0 [sh1entryaddr (Hs & HlookupCurrs0 & HlookupBTDs0 & HstartBTDPs0 & HBTDNotPart &
+      HblocksInCurr & HcurrIsPart & HcurrIsPDT & Hsh1s0 & Hpropss0 & HgtNIdx & HltIdxKernEntrieNb & HkernIsKSs0 &
+      HcurrBlock & Hstarts0 & Hends0 & HPDchilds0 & HpropsAddrToRemove)]]].
+    set(newBentry:= CBlockEntry (read bentry0) (write bentry0) (exec bentry0) (present bentry0) true
+      (blockindex bentry0) (blockrange bentry0)). fold newBentry in Hs. unfold CBlockEntry in *.
+    assert(blockindex bentry0 < kernelStructureEntriesNb) by (apply Hidx).
+    destruct (Compare_dec.lt_dec (blockindex bentry0) kernelStructureEntriesNb); try(lia).
+    assert(HkernIsKS: isKS kernel s).
+    {
+      unfold isKS in *. rewrite Hs. simpl. destruct (beqAddr currBlock kernel) eqn:HbeqCurrKern.
+      - rewrite <-beqAddrTrue in HbeqCurrKern. subst kernel. rewrite HlookupCurrs0 in *. auto.
+      - rewrite <-beqAddrFalse in *. rewrite removeDupIdentity; auto.
+    }
+    assert(Hstart: bentryStartAddr currBlock startBlock s).
+    {
+      unfold bentryStartAddr in *. rewrite HlookupCurrs0 in *. rewrite Hs. simpl. rewrite IL.beqAddrTrue. auto.
+    }
+    assert(Hend: bentryEndAddr currBlock endBlock s).
+    {
+      unfold bentryEndAddr in *. rewrite HlookupCurrs0 in *. rewrite Hs. simpl. rewrite IL.beqAddrTrue. auto.
+    }
+    assert(HPDchild: sh1entryPDchild sh1entryaddr blockToDelete s).
+    {
+      unfold sh1entryPDchild in *. rewrite Hs. simpl. destruct (beqAddr currBlock sh1entryaddr) eqn:HbeqCurrSh1.
+      { rewrite <-beqAddrTrue in HbeqCurrSh1. rewrite HbeqCurrSh1 in *. rewrite HlookupCurrs0 in *. congruence. }
+      rewrite <-beqAddrFalse in *. rewrite removeDupIdentity; auto.
+    }
+    assert(HlookupBTD: lookup blockToDelete (memory s) beqAddr = None).
+    {
+      rewrite Hs. simpl. destruct (beqAddr currBlock blockToDelete) eqn:HbeqCBBTD.
+      { rewrite <-beqAddrTrue in HbeqCBBTD. subst blockToDelete. congruence. }
+      rewrite <-beqAddrFalse in *. rewrite removeDupIdentity; auto.
+    }
+    assert(bentryStartAddr blockTDParent blockToDelete s).
+    {
+      unfold bentryStartAddr in *. rewrite Hs. simpl. destruct (beqAddr currBlock blockTDParent) eqn:HbeqCurrBBTDP.
+      - rewrite <-beqAddrTrue in HbeqCurrBBTDP. subst blockTDParent. rewrite HlookupCurrs0 in *. auto.
+      - rewrite <-beqAddrFalse in *. rewrite removeDupIdentity; auto.
+    }
+    instantiate(1 := fun s => S n > currIdx /\ currIdx < kernelStructureEntriesNb
+      /\ currBlock = CPaddr (kernel + currIdx)
+      /\ isKS kernel s
+      /\ bentryStartAddr currBlock startBlock s
+      /\ bentryEndAddr currBlock endBlock s
+      /\ lookup blockToDelete (memory s) beqAddr = None
+      /\ bentryStartAddr blockTDParent blockToDelete s
+      /\ exists s0 bentry0 sh1entryaddr newBentry,
+          deleteProps s0 blockTDParent blockToDelete
+          /\ s = {|
+                   currentPartition := currentPartition s0; memory := add currBlock (BE newBentry) (memory s0) beqAddr
+                 |}
+          /\ (exists l,
+                newBentry = {|
+                              read := read bentry0;
+                              write := write bentry0;
+                              exec := exec bentry0;
+                              present := present bentry0;
+                              accessible := true;
+                              blockindex := blockindex bentry0;
+                              blockrange := blockrange bentry0;
+                              Hidx := l
+                            |})
+          /\ lookup currBlock (memory s0) beqAddr = Some (BE bentry0)
+          /\ sh1entryaddr = CPaddr (currBlock + sh1offset)
+          /\ isKS kernel s0
+          /\ bentryStartAddr currBlock startBlock s0
+          /\ bentryEndAddr currBlock endBlock s0
+          /\ sh1entryPDchild sh1entryaddr blockToDelete s0
+          /\ sh1entryPDchild sh1entryaddr blockToDelete s
+          /\ lookup blockToDelete (memory s0) beqAddr = None
+          /\ bentryStartAddr blockTDParent blockToDelete s0
+          /\ ~ In blockToDelete (getPartitions multiplexer s0)
+          /\ (forall blockIdx, blockIdx < kernelStructureEntriesNb
+                -> In (CPaddr (kernel+blockIdx)) (filterOptionPaddr (getKSEntries currentPart s0)))
+          /\ In currentPart (getPartitions multiplexer s0)
+          /\ isPDT currentPart s0
+          /\ (forall block startBlock endBlock, In block (getMappedBlocks currentPart s0)
+                -> sh1entryPDchild (CPaddr (block+sh1offset)) blockToDelete s0
+                -> bentryStartAddr block startBlock s0
+                -> bentryEndAddr block endBlock s0
+                -> (forall addr, In addr (getAllPaddrBlock startBlock endBlock)
+                    -> ~In addr (getPartitions multiplexer s0)
+                        /\ (forall part, In part (getPartitions multiplexer s0)
+                            -> ~In addr (filterOptionPaddr (getKSEntries part s0))
+                                /\ ~In addr (getConfigPaddr part s0))
+                        /\ (isBE addr s0 -> addr + scoffset < endBlock)
+                        /\ (isKS addr s0 -> addr + nextoffset < endBlock)
+                        /\ addr <> nullAddr))).
+    intuition.
+    - exists s0. exists bentry0. exists sh1entryaddr. exists newBentry. intuition.
+      exists (ADT.CBlockEntry_obligation_1 (blockindex bentry0) l). auto.
+    - exists newBentry. rewrite Hs at 1. simpl. rewrite IL.beqAddrTrue. split; trivial.
+      assert(HblockMinIdxIsKS: KernelStructureStartFromBlockEntryAddrIsKS s0) by (unfold deleteProps in *; intuition).
+      assert(HblkIdxCB: bentryBlockIndex currBlock (blockindex bentry0) s0).
+      { unfold bentryBlockIndex. rewrite HlookupCurrs0. reflexivity. }
+      assert(HCBIsBE: isBE currBlock s0) by (unfold isBE; rewrite HlookupCurrs0; trivial).
+      specialize(HblockMinIdxIsKS currBlock (blockindex bentry0) HCBIsBE HblkIdxCB). unfold isKS in *. rewrite Hs.
+      simpl. assert(HgebCBIdx: currBlock >= blockindex bentry0).
+      {
+        destruct (Nat.ltb currBlock (blockindex bentry0)) eqn:HltCBIdx.
+        {
+          apply PeanoNat.Nat.ltb_lt in HltCBIdx. exfalso. assert(Heq: currBlock - blockindex bentry0 = 0) by lia.
+          rewrite Heq in HblockMinIdxIsKS. assert(isPADDR nullAddr s0) by (unfold deleteProps in *; intuition).
+          fold nullAddr in HblockMinIdxIsKS. unfold isPADDR in *.
+          destruct (lookup nullAddr (memory s0) beqAddr); try(congruence). destruct v; congruence.
+        }
+        apply PeanoNat.Nat.ltb_ge in HltCBIdx. lia.
+      }
+      destruct (beqAddr currBlock (CPaddr (currBlock - blockindex bentry0))) eqn:HbeqCBIdxCB.
+      + simpl. unfold CPaddr in HbeqCBIdxCB. assert(currBlock <= maxAddr) by (apply Hp).
+        destruct (Compare_dec.le_dec (currBlock - blockindex bentry0) maxAddr); try(lia).
+        rewrite <-beqAddrTrue in HbeqCBIdxCB. apply paddrEqNatEqEquiv in HbeqCBIdxCB. simpl in *.
+        assert(HidxIsZero: i (blockindex bentry0) = 0).
+        {
+          revert HbeqCBIdxCB HgebCBIdx. generalize (i (blockindex bentry0)). intros blkidx HbeqCBIdxCB HgebCBIdx.
+          destruct blkidx; trivial. exfalso.
+          assert(currBlock - S blkidx < currBlock) by (apply PeanoNat.Nat.sub_lt; lia). lia.
+        }
+        rewrite HidxIsZero. split; try(lia). unfold zero. apply index_eq_i. cbn. assumption.
+      + rewrite <-beqAddrFalse in *. rewrite removeDupIdentity; auto.
+  }
+  intro. eapply bindRev.
+  { (** MAL.forgetBlock **)
+    eapply weaken. apply forgetBlock. intros s Hprops. apply Hprops.
+  }
+  intro forgetSucc. eapply bindRev.
+  { (** Internal.checkBlockCut **)
+    eapply weaken. apply checkBlockCut (*may need to change that*). intros s Hprops. simpl.
+    destruct Hprops as [s2 ([s1 (Hs2 & HgtNIdx & HltIdxKernEntriesNb & HcurrBlock & HkernCIsKSs1 & HstartCBs1 &
+      HendCBs1 & HlookupBTDs1 & HstartBTDPs1 & [s0 [bentry0 [sh1entryaddr [newBentry (Hpropss0 & Hs1 & HnewB &
+      HlookupCurrBs0 & Hsh1CB & HkernCIsKSs0 & HstartCBs0 & HendCBs0 & HPDchildCBs0 & HPDchildCBs1 & HlookupBTDs0 &
+      HstartBTDPs0 & HBTDNotParts0 & HblocksInCurr & HcurrIsPart & HcurrIsPDT & HpropsAddrToRemove)]]]])] & HcurrEq &
+      HremovedAddrs & HlookupsEq & _)].
+
+    assert(HcurrEqss0: currentPartition s = currentPartition s2).
+    { rewrite HcurrEq. rewrite Hs2. simpl. rewrite Hs1. reflexivity. }
+    assert(Hsh1CBs0: sh1entryAddr currBlock sh1entryaddr s0).
+    { unfold sh1entryAddr. rewrite HlookupCurrBs0. assumption. }
+    assert(HCBIsBEs0: isBE currBlock s0).
+    { unfold isBE. rewrite HlookupCurrBs0. trivial. }
+    assert(HPDflagCBs0: sh1entryPDflag sh1entryaddr false s0).
+    {
+      assert(HPDNoChild: PDflagMeansNoChild s0) by (unfold deleteProps in *; intuition). subst sh1entryaddr.
+      specialize(HPDNoChild currBlock HCBIsBEs0). unfold sh1entryPDflag in *. unfold sh1entryPDchild in *.
+      destruct (lookup (CPaddr (currBlock+sh1offset)) (memory s0) beqAddr); try(congruence).
+      destruct v; try(congruence). destruct (PDflag s3); trivial. exfalso. assert(HeqTriv: true = true) by trivial.
+      specialize(HPDNoChild HeqTriv). rewrite <-HPDNoChild in *. subst blockToDelete.
+      assert(isPADDR nullAddr s0) by (unfold deleteProps in *; intuition). unfold isPADDR in *.
+      rewrite HlookupBTDs0 in *. congruence.
+    }
+    assert(HgetPartsEqs1s0: getPartitions multiplexer s1 = getPartitions multiplexer s0).
+    {
+      rewrite Hs1. apply getPartitionsEqBEPDflagFalse with bentry0 sh1entryaddr blockTDParent blockToDelete; trivial.
+      1-3: unfold deleteProps in *; intuition.
+      unfold getPartitions. replace (maxAddr+2) with (S (maxAddr+1)); try(lia). simpl. auto.
+    }
+    assert(HgetKSEqs1s0: forall part, getKSEntries part s1 = getKSEntries part s0).
+    {
+      intro part. rewrite Hs1. apply IL.getKSEntriesEqBE; trivial.
+    }
+    destruct HnewB as [l HnewB].
+    assert(HgetMappedBEqs1s0: forall part, getMappedBlocks part s1 = getMappedBlocks part s0).
+    {
+      intro part. rewrite Hs1. apply IL.getMappedBlocksEqBENoChange with bentry0; trivial. subst newBentry.
+      reflexivity.
+    }
+    assert(HgetMappedPEqs1s0: forall part, isPDT part s0 -> getMappedPaddr part s1 = getMappedPaddr part s0).
+    {
+      intros part HpartIsPDT. rewrite Hs1.
+      apply IL.getMappedPaddrEqBEPresentNoChangeStartNoChangeEndNoChangeEquivalence with bentry0; subst newBentry;
+        auto.
+    }
+    assert(HbeqBTDNull: blockToDelete <> nullAddr).
+    {
+      intro. subst blockToDelete. assert(isPADDR nullAddr s0) by (unfold deleteProps in *; intuition).
+      unfold isPADDR in *. rewrite HlookupBTDs0 in *. congruence.
+    }
+    assert(HCBInCurrs0: In currBlock (filterOptionPaddr (getKSEntries currentPart s0))).
+    { subst currBlock. apply HblocksInCurr; assumption. }
+    assert(HgetAccMappedBEqs1s0: forall part, isPDT part s0 -> currentPart <> part
+      -> getAccessibleMappedBlocks part s1 = getAccessibleMappedBlocks part s0).
+    {
+      intros part HpartIsPDT HbeqCurrPart. rewrite Hs1. apply IL.getAccessibleMappedBlocksEqBENotInPart; trivial.
+      assert(Hdisjoint: DisjointKSEntries s0) by (unfold deleteProps in *; intuition).
+      specialize(Hdisjoint currentPart part HcurrIsPDT HpartIsPDT HbeqCurrPart).
+      destruct Hdisjoint as [list1 [list2 (Hlist1 & Hlist2 & Hdisjoint)]]. subst list1. subst list2.
+      specialize(Hdisjoint currBlock HCBInCurrs0). assumption.
+    }
+    assert(HgetAccMappedBEqCurrs1s0: accessible bentry0 = true
+      -> getAccessibleMappedBlocks currentPart s1 = getAccessibleMappedBlocks currentPart s0).
+    {
+      intro Haccess. rewrite Hs1.
+      apply IL.getAccessibleMappedBlocksEqBEAccessiblePresentNoChange with bentry0; trivial; subst newBentry;
+        auto.
+    }
+    assert(HPflagCBs0: bentryPFlag currBlock true s0).
+    {
+      assert(Hres: sharedBlockIsPresent s0) by (unfold deleteProps in *; intuition). unfold sharedBlockIsPresent in *.
+      subst sh1entryaddr. apply Hres with currentPart blockToDelete; trivial.
+    }
+    assert(HgetAccMappedBImplCurrs1s0: accessible bentry0 = false
+      -> forall block, In block (getAccessibleMappedBlocks currentPart s1)
+          <-> In block (currBlock::getAccessibleMappedBlocks currentPart s0)).
+    {
+      intros Haccess block. rewrite Hs1.
+      apply IL.getAccessibleMappedBlocksEqBEPresentTrueNoChangeAccessibleTrueChangeEquivalence with bentry0; trivial.
+      1-4: rewrite HnewB; auto.
+      - unfold bentryPFlag in *. rewrite HlookupCurrBs0 in *. auto.
+      - rewrite Haccess. simpl. intro; congruence.
+      - unfold deleteProps in *; intuition.
+    }
+    assert(HgetAccMappedPEqs1s0: forall part, isPDT part s0 -> currentPart <> part
+      -> getAccessibleMappedPaddr part s1 = getAccessibleMappedPaddr part s0).
+    {
+      intros part HpartIsPDT HbeqCurrPart. rewrite Hs1. apply IL.getAccessibleMappedPaddrEqBENotInPart; trivial.
+      assert(Hdisjoint: DisjointKSEntries s0) by (unfold deleteProps in *; intuition).
+      specialize(Hdisjoint currentPart part HcurrIsPDT HpartIsPDT HbeqCurrPart).
+      destruct Hdisjoint as [list1 [list2 (Hlist1 & Hlist2 & Hdisjoint)]]. subst list1. subst list2.
+      specialize(Hdisjoint currBlock HCBInCurrs0). assumption.
+    }
+    assert(HgetAccMappedPEqCurrs1s0: accessible bentry0 = true
+      -> getAccessibleMappedPaddr currentPart s1 = getAccessibleMappedPaddr currentPart s0).
+    {
+      intro Haccess. rewrite Hs1.
+      apply IL.getAccessibleMappedPaddrEqBEPresentAccessibleNoChange with bentry0; trivial; subst newBentry;
+        auto.
+    }
+    assert(HgetAccMappedPImplCurrs1s0: accessible bentry0 = false
+      -> forall addr, In addr (getAccessibleMappedPaddr currentPart s1)
+          <-> In addr (getAllPaddrBlock startBlock endBlock ++ getAccessibleMappedPaddr currentPart s0)).
+    {
+      unfold bentryStartAddr in *. unfold bentryEndAddr in *. rewrite HlookupCurrBs0 in *. rewrite HstartCBs0.
+      rewrite HendCBs0. intros Haccess addr. rewrite Hs1.
+      apply IL.getAccessibleMappedPaddrEqBEPresentTrueNoChangeAccessibleTrueChangeEquivalence; trivial.
+      1-6: rewrite HnewB; auto.
+      - unfold bentryPFlag in *. rewrite HlookupCurrBs0 in *. auto.
+      - rewrite Haccess. simpl. intro; congruence.
+      - unfold deleteProps in *; intuition.
+    }
+    assert(HgetConfigEqs1s0: forall part, isPDT part s0 -> getConfigPaddr part s1 = getConfigPaddr part s0).
+    {
+      intros part HpartIsPDT. rewrite Hs1. apply IL.getConfigPaddrEqBE; trivial.
+    }
+    assert(HbeqCBNull: currBlock <> nullAddr).
+    {
+      intro Hcontra. rewrite Hcontra in *. assert(isPADDR nullAddr s0) by (unfold deleteProps in *; intuition).
+      unfold isPADDR in *. rewrite HlookupCurrBs0 in *. congruence.
+    }
+    assert(HcurrBNotFrees0: forall part, isPDT part s0
+      -> ~In currBlock (filterOptionPaddr (getFreeSlotsList part s0))).
+    {
+      intros part HpartIsPDT. assert(HwellFree: getFreeSlotsList part s0 = getFreeSlotsList part s0
+        /\ wellFormedFreeSlotsList (getFreeSlotsList part s0) <> False).
+      {
+        split; trivial. assert(Hres: NoDupInFreeSlotsList s0) by (unfold deleteProps in *; intuition).
+        unfold isPDT in *. destruct (lookup part (memory s0) beqAddr) eqn:HlookupPart; try(exfalso; congruence).
+        destruct v; try(exfalso; congruence). specialize(Hres part p HlookupPart).
+        destruct Hres as [optFree (HoptFree & Hres & _)]. subst optFree. assumption.
+      }
+      assert(HfreeAreFree: freeSlotsListIsFreeSlot s0) by (unfold deleteProps in *; intuition). intro Hcontra.
+      assert(HCBIsFree: filterOptionPaddr (getFreeSlotsList part s0) = filterOptionPaddr (getFreeSlotsList part s0)
+        /\ In currBlock (filterOptionPaddr (getFreeSlotsList part s0))) by auto.
+      specialize(HfreeAreFree part currBlock (getFreeSlotsList part s0) (filterOptionPaddr (getFreeSlotsList part s0))
+        HpartIsPDT HwellFree HCBIsFree HbeqCBNull). unfold isFreeSlot in *. unfold bentryPFlag in *.
+      rewrite HlookupCurrBs0 in *. rewrite <-HPflagCBs0 in *.
+      destruct (lookup (CPaddr (currBlock+sh1offset)) (memory s0) beqAddr); try(congruence).
+      destruct v; try(congruence).
+      destruct (lookup (CPaddr (currBlock+scoffset)) (memory s0) beqAddr); try(congruence).
+      destruct v; try(congruence). destruct HfreeAreFree as (_ & _ & _ & _ & HcontraB & _). congruence.
+    }
+    assert(HgetFreeEqs1s0: forall part, getFreeSlotsList part s1 = getFreeSlotsList part s0).
+    {
+      intro part. rewrite Hs1. unfold getFreeSlotsList in *. specialize(HcurrBNotFrees0 part). simpl lookup.
+      destruct (beqAddr currBlock part) eqn:HbeqCurrBPart.
+      - rewrite <-beqAddrTrue in HbeqCurrBPart. subst part. rewrite HlookupCurrBs0. reflexivity.
+      - rewrite <-beqAddrFalse in *. rewrite removeDupIdentity; auto.
+        assert(HfreeProps: NoDupInFreeSlotsList s0) by (unfold deleteProps in *; intuition).
+        destruct (lookup part (memory s0) beqAddr) eqn:HlookupPart; trivial. destruct v; trivial.
+        specialize(HfreeProps part p HlookupPart).
+        destruct HfreeProps as [optFree (HoptFree & HwellFree & HnoDupFree)]. subst optFree.
+        assert(HpartIsPDT: isPDT part s0) by (unfold isPDT; rewrite HlookupPart; trivial).
+        specialize(HcurrBNotFrees0 HpartIsPDT). unfold getFreeSlotsList in *. rewrite HlookupPart in *.
+        destruct (beqAddr (firstfreeslot p) nullAddr) eqn:HbeqFirstNull; trivial.
+        apply IL.getFreeSlotsListRecEqBE; trivial. intro Hcontra. rewrite <-Hcontra in *. contradict HcurrBNotFrees0.
+        assert(HeqTriv: getFreeSlotsList part s0 = getFreeSlotsList part s0) by trivial. rewrite <-beqAddrFalse in *.
+        assert(HfirstIsFree: FirstFreeSlotPointerIsBEAndFreeSlot s0) by (unfold deleteProps in *; intuition).
+        assert(HnbFree: pdentryNbFreeSlots part (nbfreeslots p) s0).
+        { unfold pdentryNbFreeSlots. rewrite HlookupPart. reflexivity. }
+        assert(Hlen: length (getFreeSlotsList part s0) = nbfreeslots p).
+        {
+          assert(Hres: NbFreeSlotsISNbFreeSlotsInList s0) by (unfold deleteProps in *; intuition).
+          specialize(Hres part (nbfreeslots p) HpartIsPDT HnbFree).
+          destruct Hres as [optFree (Heq & _ & Hres)]. subst optFree. auto.
+        }
+        pose proof (firstFreeSlotPointerIsFirstFreeLight part s0 p (getFreeSlotsList part s0) (nbfreeslots p)
+          HeqTriv HlookupPart HbeqFirstNull Hlen HnbFree HfirstIsFree) as Hres.
+        destruct Hres as [remainsSlotsList [_ [_ (Hres & _)]]]. unfold getFreeSlotsList in *.
+        rewrite HlookupPart in *. rewrite beqAddrFalse in *. rewrite HbeqFirstNull in *. rewrite Hres. simpl. auto.
+    }
+    assert(HgetChildrenEqs1s0: forall part, isPDT part s0 -> getChildren part s1 = getChildren part s0).
+    {
+      intros part HpartIsPart. rewrite Hs1. apply IL.getChildrenEqBENoStartNoPresentChange with bentry0; trivial;
+        rewrite HnewB; auto.
+    }
+    assert(HgetAllPaddrAuxEqs1s0: forall block, getAllPaddrAux [block] s1 = getAllPaddrAux [block] s0).
+    {
+      intro block. rewrite Hs1. simpl. destruct (beqAddr currBlock block) eqn:HbeqBlocks.
+      - rewrite <-beqAddrTrue in HbeqBlocks. subst block. rewrite HlookupCurrBs0. rewrite HnewB. reflexivity.
+      - rewrite <-beqAddrFalse in *. rewrite removeDupIdentity; auto.
+    }
+    assert(Hnulls1: nullAddrExists s1).
+    { (* BEGIN nullAddr s1 *)
+      unfold nullAddrExists. assert(Hcons0: isPADDR nullAddr s0) by (unfold deleteProps in *; intuition).
+      unfold isPADDR in *. rewrite Hs1. simpl. destruct (beqAddr currBlock nullAddr) eqn:HbeqCurrBNull.
+      {
+        rewrite <-beqAddrTrue in HbeqCurrBNull. rewrite HbeqCurrBNull in *. rewrite HlookupCurrBs0 in *. congruence.
+      }
+      rewrite <-beqAddrFalse in *. rewrite removeDupIdentity; auto.
+      (* END nullAddrExists *)
+    }
+    assert(HCBInCurrs1: In currBlock (filterOptionPaddr (getKSEntries currentPart s1))).
+    { rewrite HgetKSEqs1s0. assumption. }
+    assert(Hsh1CurrIsSHEs0: wellFormedFstShadowIfBlockEntry s0) by (unfold deleteProps in *; intuition).
+    specialize(Hsh1CurrIsSHEs0 currBlock HCBIsBEs0).
+    assert(HlookupSh1Eqs1s0: lookup (CPaddr (currBlock + sh1offset)) (memory s1) beqAddr
+      = lookup (CPaddr (currBlock + sh1offset)) (memory s0) beqAddr).
+    {
+      unfold isSHE in *. rewrite Hs1. simpl.
+      destruct (beqAddr currBlock (CPaddr (currBlock+sh1offset))) eqn:HbeqCBSh1.
+      {
+        rewrite <-beqAddrTrue in HbeqCBSh1. rewrite <-HbeqCBSh1 in *. rewrite HlookupCurrBs0 in *.
+        exfalso; congruence.
+      }
+      rewrite <-beqAddrFalse in *. rewrite removeDupIdentity; auto.
+    }
+    assert(HgetPartsEqs2s1: getPartitions multiplexer s2 = getPartitions multiplexer s1).
+    {
+      subst sh1entryaddr. unfold sh1entryPDflag in *. rewrite <-HlookupSh1Eqs1s0 in *.
+      destruct (lookup (CPaddr (currBlock+sh1offset)) (memory s1) beqAddr) eqn:HlookupSh1; try(exfalso; congruence).
+      destruct v; try(exfalso; congruence). rewrite Hs2.
+      apply getPartitionsEqSHEPDflagNoChange with s3; trivial.
+    }
+    unfold isSHE in *. rewrite <-HlookupSh1Eqs1s0 in *.
+    assert(HgetKSEqs2s1: forall part, isPDT part s1 -> getKSEntries part s2 = getKSEntries part s1).
+    {
+      intros part HpartIsPDT. unfold isPDT in *. rewrite Hs2.
+      destruct (lookup part (memory s1) beqAddr) eqn:HlookupPart; try(exfalso; congruence).
+      destruct v; try(exfalso; congruence).
+      apply IL.getKSEntriesEqSHE with p; trivial.
+    }
+    assert(HgetMappedBEqs2s1: forall part, isPDT part s1 -> getMappedBlocks part s2 = getMappedBlocks part s1).
+    {
+      intros part HpartIsPDT. rewrite Hs2. apply IL.getMappedBlocksEqSHE; trivial.
+    }
+    assert(HgetMappedPEqs2s1: forall part, isPDT part s1 -> getMappedPaddr part s2 = getMappedPaddr part s1).
+    {
+      intros part HpartIsPDT. rewrite Hs2. apply IL.getMappedPaddrEqSHE; trivial.
+    }
+    assert(HgetAccMappedBEqs2s1: forall part, isPDT part s1
+      -> getAccessibleMappedBlocks part s2 = getAccessibleMappedBlocks part s1).
+    {
+      intros part HpartIsPDT. rewrite Hs2. apply IL.getAccessibleMappedBlocksEqSHE; trivial.
+    }
+    assert(HgetAccMappedPEqs2s1: forall part, isPDT part s1
+      -> getAccessibleMappedPaddr part s2 = getAccessibleMappedPaddr part s1).
+    {
+      intros part HpartIsPDT. rewrite Hs2. apply IL.getAccessibleMappedPaddrEqSHE; trivial.
+    }
+    assert(HgetChildrenEqs2s1: forall part, isPDT part s1 -> getChildren part s2 = getChildren part s1).
+    {
+      subst sh1entryaddr. unfold sh1entryPDflag in *. rewrite <-HlookupSh1Eqs1s0 in *.
+      destruct (lookup (CPaddr (currBlock+sh1offset)) (memory s1) beqAddr) eqn:HlookupSh1; try(exfalso; congruence).
+      destruct v; try(exfalso; congruence).
+      intros part HpartIsPDT. rewrite Hs2. apply IL.getChildrenEqSHE with s3; trivial.
+    }
+    assert(HfirstIsFrees1: FirstFreeSlotPointerIsBEAndFreeSlot s1).
+    { (* BEGIN FirstFreeSlotPointerIsBEAndFreeSlot s1 *)
+      assert(Hcons0: FirstFreeSlotPointerIsBEAndFreeSlot s0) by (unfold deleteProps in *; intuition).
+      intros part pdentry HlookupPart HbeqFirstNull. rewrite Hs1 in HlookupPart. simpl in *.
+      destruct (beqAddr currBlock part) eqn:HbeqCurrBPart; try(exfalso; congruence). rewrite <-beqAddrFalse in *.
+      rewrite removeDupIdentity in *; auto. specialize(Hcons0 part pdentry HlookupPart HbeqFirstNull).
+      destruct Hcons0 as (HfirstIsBE & HfirstIsFree). unfold isBE in *. unfold isFreeSlot in *. rewrite Hs1 at 1.
+      rewrite Hs1 at 1. simpl. destruct (beqAddr currBlock (firstfreeslot pdentry)) eqn:HbeqCurrBFirst.
+      {
+        exfalso. rewrite <-beqAddrTrue in HbeqCurrBFirst. rewrite <-HbeqCurrBFirst in *. rewrite <-Hsh1CB in *.
+        rewrite HlookupCurrBs0 in *. unfold sh1entryPDchild in *.
+        destruct (lookup sh1entryaddr (memory s0) beqAddr); try(congruence). destruct v; try(congruence).
+        rewrite <-HPDchildCBs0 in *.
+        destruct (lookup (CPaddr (currBlock+scoffset)) (memory s0) beqAddr); try(congruence).
+        destruct v; try(congruence). destruct HfirstIsFree as (_ & _ & _ & _ & _ & _ & Hcontra & _).
+        rewrite Hcontra in *. unfold nullAddrExists in *. unfold isPADDR in *. rewrite HlookupBTDs1 in *. congruence.
+      }
+      rewrite <-beqAddrFalse in *. rewrite removeDupIdentity; auto. split; trivial.
+      destruct (lookup (firstfreeslot pdentry) (memory s0) beqAddr); try(congruence). destruct v; try(congruence).
+      rewrite Hs1. simpl. destruct (beqAddr currBlock (CPaddr (firstfreeslot pdentry + sh1offset))) eqn:HbeqCBSh1.
+      {
+        rewrite <-beqAddrTrue in HbeqCBSh1. rewrite <-HbeqCBSh1 in *. rewrite HlookupCurrBs0 in *. congruence.
+      }
+      rewrite <-beqAddrFalse in *. rewrite removeDupIdentity; auto.
+      destruct (lookup (CPaddr (firstfreeslot pdentry + sh1offset)) (memory s0) beqAddr); try(congruence).
+      destruct v; try(congruence).
+      destruct (beqAddr currBlock (CPaddr (firstfreeslot pdentry+scoffset))) eqn:HbeqCBSce.
+      {
+        rewrite <-beqAddrTrue in HbeqCBSce. rewrite <-HbeqCBSce in *. rewrite HlookupCurrBs0 in *. congruence.
+      }
+      rewrite <-beqAddrFalse in *. rewrite removeDupIdentity; auto.
+      (* END FirstFreeSlotPointerIsBEAndFreeSlot *)
+    }
+    assert(HgetFreeEqs2s1: forall part, getFreeSlotsList part s2 = getFreeSlotsList part s1).
+    {
+      intro part. rewrite Hs2. unfold getFreeSlotsList. simpl lookup.
+      destruct (beqAddr (CPaddr (currBlock + sh1offset)) part) eqn:HbeqSh1Part.
+      - rewrite <-beqAddrTrue in HbeqSh1Part. subst part. unfold isSHE in *.
+        destruct (lookup (CPaddr (currBlock + sh1offset)) (memory s1) beqAddr); try(exfalso; congruence).
+        destruct v; try(exfalso; congruence). reflexivity.
+      - rewrite <-beqAddrFalse in *. rewrite removeDupIdentity; auto.
+        destruct (lookup part (memory s1) beqAddr) eqn:HlookupPart; trivial. destruct v; trivial.
+        destruct (beqAddr (firstfreeslot p) nullAddr) eqn:HbeqFirstNull; trivial. unfold isSHE in *.
+        apply IL.getFreeSlotsListRecEqSHE; trivial.
+        2,3: unfold isBE; unfold isPADDR; destruct (lookup (CPaddr (currBlock+sh1offset)) (memory s1) beqAddr);
+          try(exfalso; congruence); destruct v; try(exfalso; congruence); auto.
+        rewrite <-beqAddrFalse in *. specialize(HfirstIsFrees1 part p HlookupPart HbeqFirstNull).
+        destruct HfirstIsFrees1 as (HfirstIsBE & _). unfold isBE in *. intro Hcontra. rewrite <-Hcontra in *.
+        destruct (lookup (firstfreeslot p) (memory s1) beqAddr); try(congruence). destruct v; congruence.
+    }
+    assert(HgetConfigEqs2s1: forall part, isPDT part s1 -> getConfigPaddr part s2 = getConfigPaddr part s1).
+    {
+      intros part HpartIsPDT. rewrite Hs2. apply IL.getConfigPaddrEqSHE; trivial.
+    }
+    assert(Hwell: wellFormedBlock s0) by (unfold deleteProps in *; intuition).
+    specialize(Hwell currBlock startBlock endBlock HPflagCBs0 HstartCBs0 HendCBs0).
+    destruct Hwell as (HltStartEndCB & HlebMinSizeCB).
+    assert(HpropsAddrToRemoveCopy: forall block startBlock endBlock, In block (getMappedBlocks currentPart s0)
+      -> sh1entryPDchild (CPaddr (block+sh1offset)) blockToDelete s0
+      -> bentryStartAddr block startBlock s0
+      -> bentryEndAddr block endBlock s0
+      -> (forall addr, In addr (getAllPaddrBlock startBlock endBlock)
+          -> ~In addr (getPartitions multiplexer s0)
+              /\ (forall part, In part (getPartitions multiplexer s0)
+                  -> ~In addr (filterOptionPaddr (getKSEntries part s0))
+                      /\ ~In addr (getConfigPaddr part s0))
+              /\ (isBE addr s0 -> addr + scoffset < endBlock)
+              /\ (isKS addr s0 -> addr + nextoffset < endBlock)
+              /\ addr <> nullAddr)) by assumption.
+    assert(HCBMapped: In currBlock (getMappedBlocks currentPart s0)).
+    {
+      unfold getMappedBlocks. unfold bentryPFlag in *. rewrite HlookupCurrBs0 in *.
+      apply IL.presentIsInFilterPresent with bentry0; auto.
+    }
+    rewrite Hsh1CB in HPDchildCBs0.
+    specialize(HpropsAddrToRemoveCopy currBlock startBlock endBlock HCBMapped HPDchildCBs0 HstartCBs0 HendCBs0).
+    assert(HgetPartsEqs2s0: getPartitions multiplexer s2 = getPartitions multiplexer s0).
+    { rewrite <-HgetPartsEqs1s0. assumption. }
+    assert(Hnulls2: isPADDR nullAddr s2).
+    {
+      unfold nullAddrExists in *. unfold isPADDR in *. rewrite Hs2. simpl.
+      destruct (beqAddr (CPaddr (currBlock + sh1offset)) nullAddr) eqn:HbeqSh1Null.
+      {
+        rewrite <-beqAddrTrue in HbeqSh1Null. rewrite HbeqSh1Null in *.
+        destruct (lookup nullAddr (memory s1) beqAddr); try(congruence). destruct v; congruence.
+      }
+      rewrite <-beqAddrFalse in *. rewrite removeDupIdentity; auto.
+    }
+    assert(Hstructs2: StructurePointerIsKS s2).
+    {
+      assert(Hcons0: StructurePointerIsKS s0) by (unfold deleteProps in *; intuition).
+      intros part pdentry HlookupPart HbeqStructNull. rewrite Hs2 in HlookupPart. simpl in *.
+      destruct (beqAddr (CPaddr (currBlock + sh1offset)) part) eqn:HbeqSh1Part; try(exfalso; congruence).
+      rewrite <-beqAddrFalse in *. rewrite removeDupIdentity in *; auto. rewrite Hs1 in HlookupPart. simpl in *.
+      destruct (beqAddr currBlock part) eqn:HbeqCBPart; try(exfalso; congruence).
+      rewrite <-beqAddrFalse in *. rewrite removeDupIdentity in *; auto.
+      specialize(Hcons0 part pdentry HlookupPart HbeqStructNull). unfold isKS in *. rewrite Hs2. simpl.
+      destruct (beqAddr (CPaddr (currBlock + sh1offset)) (structure pdentry)) eqn:HbeqSh1Struct.
+      {
+        rewrite HlookupSh1Eqs1s0 in *. rewrite <-beqAddrTrue in HbeqSh1Struct. rewrite HbeqSh1Struct in *.
+        destruct (lookup (structure pdentry) (memory s0) beqAddr); try(congruence). destruct v; congruence.
+      }
+      rewrite <-beqAddrFalse in *. rewrite removeDupIdentity; auto. rewrite Hs1. simpl.
+      destruct (beqAddr currBlock (structure pdentry)) eqn:HbeqCBStruct.
+      - rewrite <-beqAddrTrue in HbeqCBStruct. rewrite <-HbeqCBStruct in *. rewrite HlookupCurrBs0 in *.
+        rewrite HnewB. auto.
+      - rewrite <-beqAddrFalse in *. rewrite removeDupIdentity; auto.
+    }
+    assert(HnextPropss2: nextKernelIsValid s2).
+    {
+      assert(Hcons0: nextKernelIsValid s0) by (unfold deleteProps in *; intuition).
+      intros kern HkernIsKS. assert(HkernIsKSs0: isKS kern s0).
+      {
+        unfold isKS in *. rewrite Hs2 in HkernIsKS. simpl in *.
+        destruct (beqAddr (CPaddr (currBlock + sh1offset)) kern) eqn:HbeqSh1Kern; try(exfalso; congruence).
+        rewrite <-beqAddrFalse in *. rewrite removeDupIdentity in *; auto. rewrite Hs1 in HkernIsKS. simpl in *.
+        destruct (beqAddr currBlock kern) eqn:HbeqCBKern.
+        - rewrite <-beqAddrTrue in HbeqCBKern. subst kern. rewrite HlookupCurrBs0. subst newBentry. auto.
+        - rewrite <-beqAddrFalse in *. rewrite removeDupIdentity in *; auto.
+      }
+      specialize(Hcons0 kern HkernIsKSs0). destruct Hcons0 as (HlebNextMax & [nextAddr (HlookupNext & HnextProps)]).
+      split; trivial. exists nextAddr. split.
+      - intro Hp. specialize(HlookupNext Hp). rewrite Hs2. simpl.
+        destruct (beqAddr (CPaddr (currBlock + sh1offset)) {| p := kern + nextoffset; Hp := Hp |}) eqn:HbeqSh1Next.
+        {
+          rewrite HlookupSh1Eqs1s0 in *. rewrite <-beqAddrTrue in HbeqSh1Next. rewrite HbeqSh1Next in *.
+          rewrite HlookupNext in *. exfalso; congruence.
+        }
+        rewrite <-beqAddrFalse in *. rewrite removeDupIdentity; auto. rewrite Hs1. simpl.
+        destruct (beqAddr currBlock {| p := kern + nextoffset; Hp := Hp |}) eqn:HbeqCBNext.
+        { rewrite <-beqAddrTrue in HbeqCBNext. exfalso; congruence. }
+        rewrite <-beqAddrFalse in *. rewrite removeDupIdentity; auto.
+      - destruct HnextProps as [HnextIsKS | HnextIsNull]; auto. left. unfold isKS in *. rewrite Hs2. simpl.
+        destruct (beqAddr (CPaddr (currBlock + sh1offset)) nextAddr) eqn:HbeqSh1Next.
+        {
+          rewrite HlookupSh1Eqs1s0 in *. rewrite <-beqAddrTrue in HbeqSh1Next. rewrite HbeqSh1Next in *.
+          destruct (lookup nextAddr (memory s0) beqAddr); try(congruence). destruct v; congruence.
+        }
+        rewrite <-beqAddrFalse in *. rewrite removeDupIdentity; auto. rewrite Hs1. simpl.
+        destruct (beqAddr currBlock nextAddr) eqn:HbeqCBNext.
+        + rewrite <-beqAddrTrue in HbeqCBNext. rewrite HbeqCBNext in *. rewrite HlookupCurrBs0 in *.
+          rewrite HnewB. auto.
+        + rewrite <-beqAddrFalse in *. rewrite removeDupIdentity; auto.
+    }
+    assert(HmaxPrepIsMaxLen: maxNbPrepareIsMaxNbKernels s2).
+    {
+      assert(Hcons0: maxNbPrepareIsMaxNbKernels s0) by (unfold deleteProps in *; intuition).
+      intros part kernList HkernList. rewrite Hs2 in HkernList. apply IL.isListOfKernelsEqSHE in HkernList.
+      rewrite Hs1 in HkernList. apply IL.isListOfKernelsEqBE in HkernList. specialize(Hcons0 part kernList HkernList).
+      assumption.
+    }
+    assert(HblkidxIsBEs2: BlocksRangeFromKernelStartIsBE s2).
+    {
+      assert(Hcons0: BlocksRangeFromKernelStartIsBE s0) by (unfold deleteProps in *; intuition).
+      intros kern idx HkernIsKS HltIdxKSNb. assert(HkernIsKSs0: isKS kern s0).
+      {
+        unfold isKS in *. rewrite Hs2 in HkernIsKS. simpl in *.
+        destruct (beqAddr (CPaddr (currBlock + sh1offset)) kern) eqn:HbeqSh1Kern; try(exfalso; congruence).
+        rewrite <-beqAddrFalse in *. rewrite removeDupIdentity in *; auto. rewrite Hs1 in HkernIsKS. simpl in *.
+        destruct (beqAddr currBlock kern) eqn:HbeqCBKern.
+        - rewrite <-beqAddrTrue in HbeqCBKern. subst kern. rewrite HlookupCurrBs0. subst newBentry. auto.
+        - rewrite <-beqAddrFalse in *. rewrite removeDupIdentity in *; auto.
+      }
+      specialize(Hcons0 kern idx HkernIsKSs0 HltIdxKSNb). unfold isBE in *. rewrite Hs2. simpl.
+      destruct (beqAddr (CPaddr (currBlock + sh1offset)) (CPaddr (kern + idx))) eqn:HbeqSh1Block.
+      {
+        rewrite HlookupSh1Eqs1s0 in *. rewrite <-beqAddrTrue in HbeqSh1Block. rewrite HbeqSh1Block in *.
+        destruct (lookup (CPaddr (kern + idx)) (memory s0) beqAddr); try(congruence). destruct v; congruence.
+      }
+      rewrite <-beqAddrFalse in *. rewrite removeDupIdentity; auto. rewrite Hs1. simpl.
+      destruct (beqAddr currBlock (CPaddr (kern + idx))) eqn:HbeqBlocks; trivial.
+      rewrite <-beqAddrFalse in *. rewrite removeDupIdentity; auto.
+    }
+    assert(HfirstIsFrees2: FirstFreeSlotPointerIsBEAndFreeSlot s2).
+    {
+      intros part pdentry HlookupPart HbeqFirstNull. rewrite Hs2 in HlookupPart. simpl in *.
+      destruct (beqAddr (CPaddr (currBlock + sh1offset)) part) eqn:HbeqSh1Part; try(exfalso; congruence).
+      rewrite <-beqAddrFalse in *. rewrite removeDupIdentity in *; auto.
+      specialize(HfirstIsFrees1 part pdentry HlookupPart HbeqFirstNull).
+      destruct HfirstIsFrees1 as (HfirstIsBE & HfirstIsFree). unfold isBE in *. unfold isFreeSlot in *. rewrite Hs2.
+      simpl. destruct (beqAddr (CPaddr (currBlock + sh1offset)) (firstfreeslot pdentry)) eqn:HbeqSh1First.
+      {
+        rewrite <-beqAddrTrue in HbeqSh1First. rewrite HbeqSh1First in *. exfalso.
+        destruct (lookup (firstfreeslot pdentry) (memory s1) beqAddr); try(congruence). destruct v; congruence.
+      }
+      rewrite <-beqAddrFalse in *. rewrite removeDupIdentity; auto. split; trivial.
+      destruct (lookup (firstfreeslot pdentry) (memory s1) beqAddr); try(congruence). destruct v; try(congruence).
+      destruct (beqAddr (CPaddr (currBlock + sh1offset)) (CPaddr (firstfreeslot pdentry + scoffset))) eqn:HbeqSh1Sce.
+      {
+        exfalso. rewrite <-beqAddrTrue in HbeqSh1Sce. rewrite HbeqSh1Sce in *.
+        destruct (lookup (CPaddr (firstfreeslot pdentry + sh1offset)) (memory s1) beqAddr); try(congruence).
+        destruct v; try(congruence).
+        destruct (lookup (CPaddr (firstfreeslot pdentry + scoffset)) (memory s1) beqAddr); try(congruence).
+        destruct v; congruence.
+      }
+      destruct (beqAddr (CPaddr (currBlock + sh1offset)) (CPaddr (firstfreeslot pdentry + sh1offset))) eqn:HbeqSh1s.
+      - rewrite <-beqAddrTrue in HbeqSh1s. rewrite <-HbeqSh1s in *.
+        destruct (lookup (CPaddr (currBlock + sh1offset)) (memory s1) beqAddr); try(exfalso; congruence).
+        destruct v; try(exfalso; congruence). rewrite <-beqAddrFalse in *. rewrite removeDupIdentity; auto.
+        destruct (lookup (CPaddr (firstfreeslot pdentry + scoffset)) (memory s1) beqAddr); try(congruence).
+        destruct v; try(congruence). intuition.
+      - rewrite <-beqAddrFalse in *. rewrite removeDupIdentity; auto. rewrite removeDupIdentity; auto.
+    }
+    assert(HwellSh1s2: wellFormedFstShadowIfBlockEntry s2).
+    {
+      assert(Hcons0: wellFormedFstShadowIfBlockEntry s0) by (unfold deleteProps in *; intuition).
+      intros block HblockIsBE. unfold isBE in *. rewrite Hs2 in HblockIsBE. simpl in *.
+      destruct (beqAddr (CPaddr (currBlock + sh1offset)) block) eqn:HbeqSh1Block; try(exfalso; congruence).
+      rewrite <-beqAddrFalse in *. rewrite removeDupIdentity in *; auto.
+      assert(HblockIsBEs0: isBE block s0).
+      {
+        unfold isBE. rewrite Hs1 in HblockIsBE. simpl in *. destruct (beqAddr currBlock block) eqn:HbeqBlocks.
+        - rewrite <-beqAddrTrue in HbeqBlocks. subst block. rewrite HlookupCurrBs0. trivial.
+        - rewrite <-beqAddrFalse in *. rewrite removeDupIdentity in *; auto.
+      }
+      specialize(Hcons0 block HblockIsBEs0). unfold isSHE in *. rewrite Hs2. simpl.
+      destruct (beqAddr (CPaddr (currBlock + sh1offset)) (CPaddr (block + sh1offset))) eqn:HbeqSh1s; trivial.
+      rewrite <-beqAddrFalse in *. rewrite removeDupIdentity; auto. rewrite Hs1. simpl.
+      destruct (beqAddr currBlock (CPaddr (block + sh1offset))) eqn:HbeqCBSh1.
+      {
+        rewrite <-beqAddrTrue in HbeqCBSh1. rewrite <-HbeqCBSh1 in *. rewrite HlookupCurrBs0 in *. congruence.
+      }
+      rewrite <-beqAddrFalse in *. rewrite removeDupIdentity; auto.
+    }
+    assert(HnoDupTrees2: noDupPartitionTree s2).
+    { unfold noDupPartitionTree. rewrite HgetPartsEqs2s0. unfold deleteProps in *; intuition. }
+    assert(HpropsAddrToRemoveSpecs2: forall addr, In addr (getAllPaddrBlock startBlock endBlock)
+      -> ~In addr (getPartitions multiplexer s2)
+          /\ (forall part, In part (getPartitions multiplexer s2)
+            -> ~In addr (filterOptionPaddr (getKSEntries part s2)) /\ ~ In addr (getConfigPaddr part s2))
+          /\ (isBE addr s2 -> addr + scoffset < endBlock)
+          /\ (isKS addr s2 -> addr + nextoffset < endBlock) /\ addr <> nullAddr).
+    {
+      intros addr HaddrInRange. specialize(HpropsAddrToRemoveCopy addr HaddrInRange).
+      destruct HpropsAddrToRemoveCopy as (HaddrNotPart & HaddrNotConfig & HltSceEnd & HltNextEnd & HbeqAddrNull).
+      rewrite HgetPartsEqs2s0. split; trivial. split. 2: split; try(split); trivial.
+      - intros part HpartIsPart. specialize(HaddrNotConfig part HpartIsPart). assert(HpartIsPDT: isPDT part s0).
+        {
+          apply partitionsArePDTPartial with blockTDParent blockToDelete; trivial;
+            unfold deleteProps in *; intuition.
+        }
+        assert(isPDT part s1).
+        {
+          unfold isPDT in *. rewrite Hs1. simpl. destruct (beqAddr currBlock part) eqn:HbeqCBPart.
+          {
+            rewrite <-beqAddrTrue in HbeqCBPart. subst part. rewrite HlookupCurrBs0 in *. congruence.
+          }
+          rewrite <-beqAddrFalse in *. rewrite removeDupIdentity; auto.
+        }
+        rewrite HgetKSEqs2s1; trivial. rewrite HgetKSEqs1s0. rewrite HgetConfigEqs2s1; trivial.
+        rewrite HgetConfigEqs1s0; assumption.
+      - intro HaddrIsBE. assert(HaddrIsBEs0: isBE addr s0).
+        {
+          unfold isBE in *. rewrite Hs2 in HaddrIsBE. simpl in *.
+          destruct (beqAddr (CPaddr (currBlock + sh1offset)) addr) eqn:HbeqSh1Addr; try(exfalso; congruence).
+          rewrite <-beqAddrFalse in *. rewrite removeDupIdentity in *; auto. rewrite Hs1 in HaddrIsBE. simpl in *.
+          destruct (beqAddr currBlock addr) eqn:HbeqCBAddr.
+          - rewrite <-beqAddrTrue in HbeqCBAddr. subst addr. rewrite HlookupCurrBs0. trivial.
+          - rewrite <-beqAddrFalse in *. rewrite removeDupIdentity in *; auto.
+        }
+        apply HltSceEnd; assumption.
+      - intro HaddrIsKS. assert(HaddrIsKSs0: isKS addr s0).
+        {
+          unfold isKS in *. rewrite Hs2 in HaddrIsKS. simpl in *.
+          destruct (beqAddr (CPaddr (currBlock + sh1offset)) addr) eqn:HbeqSh1Addr; try(exfalso; congruence).
+          rewrite <-beqAddrFalse in *. rewrite removeDupIdentity in *; auto. rewrite Hs1 in HaddrIsKS. simpl in *.
+          destruct (beqAddr currBlock addr) eqn:HbeqCBAddr.
+          - rewrite <-beqAddrTrue in HbeqCBAddr. subst addr. rewrite HlookupCurrBs0. subst newBentry. auto.
+          - rewrite <-beqAddrFalse in *. rewrite removeDupIdentity in *; auto.
+        }
+        apply HltNextEnd; assumption.
+    }
+    assert(HcurrIsPDTs1: isPDT currentPart s1).
+    {
+      unfold isPDT in *. rewrite Hs1. simpl. destruct (beqAddr currBlock currentPart) eqn:HbeqCBCurr.
+      {
+        rewrite <-beqAddrTrue in HbeqCBCurr. rewrite HbeqCBCurr in *. rewrite HlookupCurrBs0 in *. congruence.
+      }
+      rewrite <-beqAddrFalse in *. rewrite removeDupIdentity; auto.
+    }
+    assert(HpropsAddrToRemoves2: forall block startBlock endBlock,
+       In block (getMappedBlocks currentPart s2)
+       -> sh1entryPDchild (CPaddr (block + sh1offset)) blockToDelete s2
+       -> bentryStartAddr block startBlock s2
+       -> bentryEndAddr block endBlock s2
+       -> forall addr, In addr (getAllPaddrBlock startBlock endBlock)
+           -> ~In addr (getPartitions multiplexer s2)
+             /\ (forall part, In part (getPartitions multiplexer s2)
+                -> ~In addr (filterOptionPaddr (getKSEntries part s2)) /\ ~ In addr (getConfigPaddr part s2))
+             /\ (isBE addr s2 -> addr + scoffset < endBlock)
+             /\ (isKS addr s2 -> addr + nextoffset < endBlock) /\ addr <> nullAddr).
+    {
+      intros block startaddr endaddr HblockMapped HPDchild Hstart Hend addr HaddrInRange.
+      rewrite HgetMappedBEqs2s1 in HblockMapped; trivial. rewrite HgetMappedBEqs1s0 in *. unfold sh1entryPDchild in *.
+      rewrite Hs2 in HPDchild. simpl in *.
+      destruct (beqAddr (CPaddr (currBlock+sh1offset)) (CPaddr (block+sh1offset))) eqn:HbeqSh1s;
+        try(simpl in *; exfalso; congruence). rewrite <-beqAddrFalse in *. rewrite removeDupIdentity in *; auto.
+      rewrite Hs1 in HPDchild. simpl in *.
+      destruct (beqAddr currBlock (CPaddr (block+sh1offset))) eqn:HbeqCBSh1; try(exfalso; congruence).
+      rewrite <-beqAddrFalse in *. rewrite removeDupIdentity in *; auto.
+      assert(Hbounds: bentryStartAddr block startaddr s0 /\ bentryEndAddr block endaddr s0).
+      {
+        unfold bentryStartAddr in *. unfold bentryEndAddr in *. rewrite Hs2 in Hstart. rewrite Hs2 in Hend.
+        simpl in *.
+        destruct (beqAddr (CPaddr (currBlock+sh1offset)) block) eqn:HbeqSh1Block; try(exfalso; congruence).
+        rewrite <-beqAddrFalse in *. rewrite removeDupIdentity in *; auto. rewrite Hs1 in Hstart. rewrite Hs1 in Hend.
+        simpl in *. destruct (beqAddr currBlock block) eqn:HbeqBlocks.
+        {
+          rewrite <-beqAddrTrue in HbeqBlocks. subst block. exfalso; congruence.
+        }
+        rewrite <-beqAddrFalse in *. rewrite removeDupIdentity in *; auto.
+      }
+      destruct Hbounds as (Hstarts0 & Hends0).
+      specialize(HpropsAddrToRemove block startaddr endaddr HblockMapped HPDchild Hstarts0 Hends0 addr HaddrInRange).
+      destruct HpropsAddrToRemove as (HaddrNotPart & HaddrNotConfig & HltSceEnd & HltNextEnd & HbeqAddrNull).
+      rewrite HgetPartsEqs2s0. split; trivial. split. 2: split; try(split); trivial.
+      - intros part HpartIsPart. specialize(HaddrNotConfig part HpartIsPart). assert(HpartIsPDT: isPDT part s0).
+        {
+          apply partitionsArePDTPartial with blockTDParent blockToDelete; trivial;
+            unfold deleteProps in *; intuition.
+        }
+        assert(isPDT part s1).
+        {
+          unfold isPDT in *. rewrite Hs1. simpl. destruct (beqAddr currBlock part) eqn:HbeqCBPart.
+          {
+            rewrite <-beqAddrTrue in HbeqCBPart. subst part. rewrite HlookupCurrBs0 in *. congruence.
+          }
+          rewrite <-beqAddrFalse in *. rewrite removeDupIdentity; auto.
+        }
+        rewrite HgetKSEqs2s1; trivial. rewrite HgetKSEqs1s0. rewrite HgetConfigEqs2s1; trivial.
+        rewrite HgetConfigEqs1s0; assumption.
+      - intro HaddrIsBE. assert(HaddrIsBEs0: isBE addr s0).
+        {
+          unfold isBE in *. rewrite Hs2 in HaddrIsBE. simpl in *.
+          destruct (beqAddr (CPaddr (currBlock + sh1offset)) addr) eqn:HbeqSh1Addr; try(exfalso; congruence).
+          rewrite <-beqAddrFalse in *. rewrite removeDupIdentity in *; auto. rewrite Hs1 in HaddrIsBE. simpl in *.
+          destruct (beqAddr currBlock addr) eqn:HbeqCBAddr.
+          - rewrite <-beqAddrTrue in HbeqCBAddr. subst addr. rewrite HlookupCurrBs0. trivial.
+          - rewrite <-beqAddrFalse in *. rewrite removeDupIdentity in *; auto.
+        }
+        apply HltSceEnd; assumption.
+      - intro HaddrIsKS. assert(HaddrIsKSs0: isKS addr s0).
+        {
+          unfold isKS in *. rewrite Hs2 in HaddrIsKS. simpl in *.
+          destruct (beqAddr (CPaddr (currBlock + sh1offset)) addr) eqn:HbeqSh1Addr; try(exfalso; congruence).
+          rewrite <-beqAddrFalse in *. rewrite removeDupIdentity in *; auto. rewrite Hs1 in HaddrIsKS. simpl in *.
+          destruct (beqAddr currBlock addr) eqn:HbeqCBAddr.
+          - rewrite <-beqAddrTrue in HbeqCBAddr. subst addr. rewrite HlookupCurrBs0. subst newBentry. auto.
+          - rewrite <-beqAddrFalse in *. rewrite removeDupIdentity in *; auto.
+        }
+        apply HltNextEnd; assumption.
+    }
+    assert(HpropsForStructEqs2: forall addr, In addr (getAllPaddrBlock startBlock endBlock)
+      -> ~In addr (getPartitions multiplexer s2)
+          /\ (forall partition, In partition (getPartitions multiplexer s2)
+              -> ~ In addr (getConfigPaddr partition s2))
+          /\ addr <> nullAddr).
+    {
+      intros addr HaddrInRange. specialize(HpropsAddrToRemoveSpecs2 addr HaddrInRange).
+      destruct HpropsAddrToRemoveSpecs2 as (HaddrNotPart & HaddrNotConfig & _ & _ & HbeqAddrNull). split; trivial.
+      split; trivial. intros part HpartIsPart. apply HaddrNotConfig; trivial.
+    }
+    assert(HgetPartsEqss0: getPartitions multiplexer s = getPartitions multiplexer s0).
+    {
+      rewrite <-HgetPartsEqs1s0. rewrite <-HgetPartsEqs2s1.
+      apply getPartitionsEqNoImpact with startBlock endBlock; trivial.
+      unfold getPartitions. replace (maxAddr+2) with (S (maxAddr+1)); try(lia). simpl. auto.
+    }
+    assert(HgetKSEqss0: forall part, In part (getPartitions multiplexer s0)
+      -> getKSEntries part s = getKSEntries part s0).
+    {
+      intros part HpartIsPart. assert(HpartIsPDT: isPDT part s0).
+      {
+        apply partitionsArePDTPartial with blockTDParent blockToDelete; trivial; unfold deleteProps in *; intuition.
+      }
+      assert(isPDT part s1).
+      {
+        unfold isPDT in *. rewrite Hs1. simpl. destruct (beqAddr currBlock part) eqn:HbeqCBPart.
+        {
+          rewrite <-beqAddrTrue in HbeqCBPart. rewrite HbeqCBPart in *. rewrite HlookupCurrBs0 in *. congruence.
+        }
+        rewrite <-beqAddrFalse in *. rewrite removeDupIdentity; auto.
+      }
+      rewrite <-HgetKSEqs1s0. rewrite <-HgetKSEqs2s1; trivial. rewrite <-HgetPartsEqs2s0 in HpartIsPart.
+      apply getKSEntriesEqNoImpact with startBlock endBlock; trivial. intros addr HaddrInRange.
+      specialize(HpropsForStructEqs2 addr HaddrInRange).
+      destruct HpropsForStructEqs2 as (HaddrNotPart & HaddrNotConfig & HbeqAddrNull). auto.
+    }
+    assert(HgetMappedBEqss0: forall part, In part (getPartitions multiplexer s0)
+      -> getMappedBlocks part s = getMappedBlocks part s0).
+    {
+      intros part HpartIsPart. assert(HpartIsPDT: isPDT part s0).
+      {
+        apply partitionsArePDTPartial with blockTDParent blockToDelete; trivial; unfold deleteProps in *; intuition.
+      }
+      assert(isPDT part s1).
+      {
+        unfold isPDT in *. rewrite Hs1. simpl. destruct (beqAddr currBlock part) eqn:HbeqCBPart.
+        {
+          rewrite <-beqAddrTrue in HbeqCBPart. rewrite HbeqCBPart in *. rewrite HlookupCurrBs0 in *. congruence.
+        }
+        rewrite <-beqAddrFalse in *. rewrite removeDupIdentity; auto.
+      }
+      rewrite <-HgetMappedBEqs1s0. rewrite <-HgetMappedBEqs2s1; trivial. rewrite <-HgetPartsEqs2s0 in HpartIsPart.
+      apply getMappedBlocksEqNoImpact with startBlock endBlock; trivial. intros addr HaddrInRange.
+      specialize(HpropsForStructEqs2 addr HaddrInRange).
+      destruct HpropsForStructEqs2 as (HaddrNotPart & HaddrNotConfig & HbeqAddrNull). auto.
+    }
+    assert(HgetMappedPEqss0: forall part, In part (getPartitions multiplexer s0)
+      -> getMappedPaddr part s = getMappedPaddr part s0).
+    {
+      intros part HpartIsPart. assert(HpartIsPDT: isPDT part s0).
+      {
+        apply partitionsArePDTPartial with blockTDParent blockToDelete; trivial; unfold deleteProps in *; intuition.
+      }
+      assert(isPDT part s1).
+      {
+        unfold isPDT in *. rewrite Hs1. simpl. destruct (beqAddr currBlock part) eqn:HbeqCBPart.
+        {
+          rewrite <-beqAddrTrue in HbeqCBPart. rewrite HbeqCBPart in *. rewrite HlookupCurrBs0 in *. congruence.
+        }
+        rewrite <-beqAddrFalse in *. rewrite removeDupIdentity; auto.
+      }
+      rewrite <-HgetMappedPEqs1s0; trivial. rewrite <-HgetMappedPEqs2s1; trivial.
+      rewrite <-HgetPartsEqs2s0 in HpartIsPart.
+      apply getMappedPaddrEqNoImpact with startBlock endBlock; trivial. intros addr HaddrInRange.
+      specialize(HpropsForStructEqs2 addr HaddrInRange).
+      destruct HpropsForStructEqs2 as (HaddrNotPart & HaddrNotConfig & HbeqAddrNull). auto.
+    }
+    assert(HgetAccMappedBEqss0NotCurr: forall part, In part (getPartitions multiplexer s0)
+      -> currentPart <> part
+      -> getAccessibleMappedBlocks part s = getAccessibleMappedBlocks part s0).
+    {
+      intros part HpartIsPart HbeqCurrPart. assert(HpartIsPDT: isPDT part s0).
+      {
+        apply partitionsArePDTPartial with blockTDParent blockToDelete; trivial; unfold deleteProps in *; intuition.
+      }
+      assert(isPDT part s1).
+      {
+        unfold isPDT in *. rewrite Hs1. simpl. destruct (beqAddr currBlock part) eqn:HbeqCBPart.
+        {
+          rewrite <-beqAddrTrue in HbeqCBPart. rewrite HbeqCBPart in *. rewrite HlookupCurrBs0 in *. congruence.
+        }
+        rewrite <-beqAddrFalse in *. rewrite removeDupIdentity; auto.
+      }
+      rewrite <-HgetAccMappedBEqs1s0; trivial. rewrite <-HgetAccMappedBEqs2s1; trivial.
+      rewrite <-HgetPartsEqs2s0 in HpartIsPart.
+      apply getAccessibleMappedBlocksEqNoImpact with startBlock endBlock; trivial. intros addr HaddrInRange.
+      specialize(HpropsForStructEqs2 addr HaddrInRange).
+      destruct HpropsForStructEqs2 as (HaddrNotPart & HaddrNotConfig & HbeqAddrNull). auto.
+    }
+    assert(HgetAccMappedPEqss0NotCurr: forall part, In part (getPartitions multiplexer s0)
+      -> currentPart <> part
+      -> getAccessibleMappedPaddr part s = getAccessibleMappedPaddr part s0).
+    {
+      intros part HpartIsPart HbeqCurrPart. assert(HpartIsPDT: isPDT part s0).
+      {
+        apply partitionsArePDTPartial with blockTDParent blockToDelete; trivial; unfold deleteProps in *; intuition.
+      }
+      assert(isPDT part s1).
+      {
+        unfold isPDT in *. rewrite Hs1. simpl. destruct (beqAddr currBlock part) eqn:HbeqCBPart.
+        {
+          rewrite <-beqAddrTrue in HbeqCBPart. rewrite HbeqCBPart in *. rewrite HlookupCurrBs0 in *. congruence.
+        }
+        rewrite <-beqAddrFalse in *. rewrite removeDupIdentity; auto.
+      }
+      rewrite <-HgetAccMappedPEqs1s0; trivial. rewrite <-HgetAccMappedPEqs2s1; trivial.
+      rewrite <-HgetPartsEqs2s0 in HpartIsPart.
+      apply getAccessibleMappedPaddrEqNoImpact with startBlock endBlock; trivial. intros addr HaddrInRange.
+      specialize(HpropsForStructEqs2 addr HaddrInRange).
+      destruct HpropsForStructEqs2 as (HaddrNotPart & HaddrNotConfig & HbeqAddrNull). auto.
+    }
+    assert(HgetAccMappedBEqCurrss0: accessible bentry0 = true
+      -> getAccessibleMappedBlocks currentPart s = getAccessibleMappedBlocks currentPart s0).
+    {
+      intro Haccess. rewrite <-HgetAccMappedBEqCurrs1s0; trivial. rewrite <-HgetAccMappedBEqs2s1; trivial.
+      rewrite <-HgetPartsEqs2s0 in HcurrIsPart.
+      apply getAccessibleMappedBlocksEqNoImpact with startBlock endBlock; trivial. intros addr HaddrInRange.
+      specialize(HpropsForStructEqs2 addr HaddrInRange).
+      destruct HpropsForStructEqs2 as (HaddrNotPart & HaddrNotConfig & HbeqAddrNull). auto.
+    }
+    assert(HgetAccMappedBImplCurrss0: accessible bentry0 = false
+      -> forall block, In block (getAccessibleMappedBlocks currentPart s)
+          <-> In block (currBlock :: getAccessibleMappedBlocks currentPart s0)).
+    {
+      intros Haccess block. specialize(HgetAccMappedBImplCurrs1s0 Haccess block).
+      rewrite <-HgetAccMappedBEqs2s1 in HgetAccMappedBImplCurrs1s0; trivial.
+      assert(Heq: getAccessibleMappedBlocks currentPart s = getAccessibleMappedBlocks currentPart s2).
+      {
+        rewrite <-HgetPartsEqs2s0 in HcurrIsPart.
+        apply getAccessibleMappedBlocksEqNoImpact with startBlock endBlock; trivial. intros addr HaddrInRange.
+        specialize(HpropsForStructEqs2 addr HaddrInRange).
+        destruct HpropsForStructEqs2 as (HaddrNotPart & HaddrNotConfig & HbeqAddrNull). auto.
+      }
+      rewrite Heq. assumption.
+    }
+    assert(HgetAccMappedPEqCurrss0: accessible bentry0 = true
+      -> getAccessibleMappedPaddr currentPart s = getAccessibleMappedPaddr currentPart s0).
+    {
+      intro Haccess. rewrite <-HgetAccMappedPEqCurrs1s0; trivial. rewrite <-HgetAccMappedPEqs2s1; trivial.
+      rewrite <-HgetPartsEqs2s0 in HcurrIsPart.
+      apply getAccessibleMappedPaddrEqNoImpact with startBlock endBlock; trivial. intros addr HaddrInRange.
+      specialize(HpropsForStructEqs2 addr HaddrInRange).
+      destruct HpropsForStructEqs2 as (HaddrNotPart & HaddrNotConfig & HbeqAddrNull). auto.
+    }
+    assert(HgetAccMappedPImplCurrss0: accessible bentry0 = false
+      -> forall addr, In addr (getAccessibleMappedPaddr currentPart s)
+          <-> In addr (getAllPaddrBlock startBlock endBlock ++ getAccessibleMappedPaddr currentPart s0)).
+    {
+      intros Haccess block. specialize(HgetAccMappedPImplCurrs1s0 Haccess block).
+      rewrite <-HgetAccMappedPEqs2s1 in HgetAccMappedPImplCurrs1s0; trivial.
+      assert(Heq: getAccessibleMappedPaddr currentPart s = getAccessibleMappedPaddr currentPart s2).
+      {
+        rewrite <-HgetPartsEqs2s0 in HcurrIsPart.
+        apply getAccessibleMappedPaddrEqNoImpact with startBlock endBlock; trivial. intros addr HaddrInRange.
+        specialize(HpropsForStructEqs2 addr HaddrInRange).
+        destruct HpropsForStructEqs2 as (HaddrNotPart & HaddrNotConfig & HbeqAddrNull). auto.
+      }
+      rewrite Heq. assumption.
+    }
+    assert(HgetConfigEqss0: forall part, In part (getPartitions multiplexer s0)
+      -> getConfigPaddr part s = getConfigPaddr part s0).
+    {
+      intros part HpartIsPart. assert(HpartIsPDT: isPDT part s0).
+      {
+        apply partitionsArePDTPartial with blockTDParent blockToDelete; trivial; unfold deleteProps in *; intuition.
+      }
+      assert(isPDT part s1).
+      {
+        unfold isPDT in *. rewrite Hs1. simpl. destruct (beqAddr currBlock part) eqn:HbeqCBPart.
+        {
+          rewrite <-beqAddrTrue in HbeqCBPart. rewrite HbeqCBPart in *. rewrite HlookupCurrBs0 in *. congruence.
+        }
+        rewrite <-beqAddrFalse in *. rewrite removeDupIdentity; auto.
+      }
+      rewrite <-HgetConfigEqs1s0; trivial. rewrite <-HgetConfigEqs2s1; trivial.
+      rewrite <-HgetPartsEqs2s0 in HpartIsPart.
+      apply getConfigPaddrEqNoImpact with startBlock endBlock; trivial. intros addr HaddrInRange.
+      specialize(HpropsForStructEqs2 addr HaddrInRange).
+      destruct HpropsForStructEqs2 as (HaddrNotPart & HaddrNotConfig & HbeqAddrNull). split; try(split); auto.
+      specialize(HaddrNotConfig part HpartIsPart). unfold getConfigPaddr in *.
+      apply Lib.in_app_or_neg in HaddrNotConfig. apply HaddrNotConfig.
+    }
+
+    assert(nullAddrExists s).
+    { (* BEGIN nullAddrExists s *)
+      unfold nullAddrExists in *. unfold isPADDR in *. rewrite HlookupsEq; trivial. intro Hcontra.
+      specialize(HpropsForStructEqs2 nullAddr Hcontra). destruct HpropsForStructEqs2 as (_ & _ & Hneq). congruence.
+      (* END nullAddrExists *)
+    }
+
+    assert(Hranges0: getAllPaddrAux [currBlock] s0 = getAllPaddrBlock startBlock endBlock).
+    {
+      simpl. unfold bentryStartAddr in *. unfold bentryEndAddr in *.
+      destruct (lookup currBlock (memory s0) beqAddr); try(exfalso; congruence). destruct v; try(exfalso; congruence).
+      rewrite <-HstartCBs0. rewrite <-HendCBs0. apply app_nil_r.
+    }
+
+    assert(Hranges1: getAllPaddrAux [currBlock] s1 = getAllPaddrBlock startBlock endBlock).
+    {
+      simpl. unfold bentryStartAddr in *. unfold bentryEndAddr in *.
+      destruct (lookup currBlock (memory s1) beqAddr); try(exfalso; congruence). destruct v; try(exfalso; congruence).
+      rewrite <-HstartCBs1. rewrite <-HendCBs1. apply app_nil_r.
+    }
+
+    assert(HlookupCBEqs2s1: lookup currBlock (memory s2) beqAddr = lookup currBlock (memory s1) beqAddr).
+    {
+      unfold bentryStartAddr in *. rewrite Hs2. simpl.
+      destruct (beqAddr (CPaddr (currBlock + sh1offset)) currBlock) eqn:HbeqNextCB.
+      {
+        rewrite <-beqAddrTrue in HbeqNextCB. rewrite HbeqNextCB in *. exfalso.
+        destruct (lookup currBlock (memory s1) beqAddr); try(congruence). destruct v; congruence.
+      }
+      rewrite <-beqAddrFalse in *. rewrite removeDupIdentity; auto.
+    }
+
+    assert(Hranges2: getAllPaddrAux [currBlock] s2 = getAllPaddrBlock startBlock endBlock).
+    {
+      unfold bentryStartAddr in *. unfold bentryEndAddr in *. simpl. rewrite HlookupCBEqs2s1.
+      destruct (lookup currBlock (memory s1) beqAddr); try(exfalso; congruence). destruct v; try(exfalso; congruence).
+      rewrite <-HstartCBs1. rewrite <-HendCBs1. apply app_nil_r.
+    }
+
+    assert(wellFormedFstShadowIfBlockEntry s).
+    { (* BEGIN wellFormedFstShadowIfBlockEntry s *)
+      intros block HblockIsBE. unfold isBE in *.
+      assert(HblockNotInRange: ~In block (getAllPaddrBlock startBlock endBlock)).
+      {
+        intro Hcontra. apply HremovedAddrs in Hcontra. rewrite Hcontra in *. congruence.
+      }
+      rewrite HlookupsEq in HblockIsBE; trivial. specialize(HwellSh1s2 block HblockIsBE). unfold isSHE in *.
+      rewrite HlookupsEq; trivial. contradict HblockNotInRange. rewrite <-Hranges0 in *.
+      assert(Hres: blockAndSh1InSameBlock s0) by (unfold deleteProps in *; intuition).
+      unfold blockAndSh1InSameBlock in *. apply Hres; assumption.
+      (* END wellFormedFstShadowIfBlockEntry *)
+    }
+
+    assert(forall idPDchild sh1entryaddr part, idPDchild <> blockTDParent
+        -> In part (getPartitions multiplexer s)
+        -> In idPDchild (getMappedBlocks part s)
+        -> true = checkChild idPDchild s sh1entryaddr /\ sh1entryAddr idPDchild sh1entryaddr s
+        -> bentryAFlag idPDchild false s /\ bentryPFlag idPDchild true s
+            /\ (exists startaddr, bentryStartAddr idPDchild startaddr s /\ entryPDT idPDchild startaddr s)).
+    { (* BEGIN PDTIfPDFlag s *)
+      assert(Hcons0: forall idPDchild sh1entryaddr part, idPDchild <> blockTDParent
+        -> In part (getPartitions multiplexer s0)
+        -> In idPDchild (getMappedBlocks part s0)
+        -> true = checkChild idPDchild s0 sh1entryaddr /\ sh1entryAddr idPDchild sh1entryaddr s0
+        -> bentryAFlag idPDchild false s0 /\ bentryPFlag idPDchild true s0
+            /\ (exists startaddr, bentryStartAddr idPDchild startaddr s0 /\ entryPDT idPDchild startaddr s0))
+        by (unfold deleteProps in *; intuition).
+      intros block sh1entryaddrB part HbeqBlockBTDP HpartIsPart HblockMapped HcheckChild.
+      rewrite HgetPartsEqss0 in *. rewrite HgetMappedBEqss0 in *; trivial.
+      assert(HlookupBlockEq: lookup block (memory s) beqAddr = lookup block (memory s1) beqAddr).
+      {
+        destruct HcheckChild as (_ & Hsh1). unfold sh1entryAddr in *.
+        assert(~ In block (getAllPaddrBlock startBlock endBlock)).
+        {
+          intro Hcontra. apply HremovedAddrs in Hcontra. rewrite Hcontra in *. congruence.
+        }
+        rewrite HlookupsEq; trivial. rewrite HlookupsEq in Hsh1; trivial. rewrite Hs2. rewrite Hs2 in Hsh1.
+        simpl in *. destruct (beqAddr (CPaddr (currBlock+sh1offset)) block) eqn:HbeqNextBlock;
+          try(exfalso; congruence). rewrite <-beqAddrFalse in *. rewrite removeDupIdentity; auto.
+      }
+      unfold checkChild in *. unfold sh1entryAddr in *. unfold bentryAFlag. unfold bentryPFlag.
+      unfold bentryStartAddr. unfold entryPDT. rewrite HlookupBlockEq in *.
+      assert(HcheckChilds0: true = checkChild block s0 sh1entryaddrB /\ sh1entryAddr block sh1entryaddrB s0).
+      {
+        unfold checkChild. unfold sh1entryAddr. destruct HcheckChild as (HcheckChild & Hsh1).
+        assert(HlookupSh1BEq: lookup sh1entryaddrB (memory s) beqAddr = lookup sh1entryaddrB (memory s0) beqAddr).
+        {
+          destruct (lookup block (memory s1) beqAddr); try(exfalso; congruence).
+          destruct v; try(exfalso; congruence). assert(~In sh1entryaddrB (getAllPaddrBlock startBlock endBlock)).
+          {
+            intro Hcontra. apply HremovedAddrs in Hcontra. rewrite Hcontra in *. congruence.
+          }
+          rewrite HlookupsEq; trivial. rewrite HlookupsEq in HcheckChild; trivial. rewrite Hs2 in HcheckChild.
+          rewrite Hs2. simpl in *. destruct (beqAddr (CPaddr (currBlock + sh1offset)) sh1entryaddrB) eqn:HbeqSh1s;
+            try(simpl in HcheckChild; exfalso; congruence). rewrite <-beqAddrFalse in *.
+          rewrite removeDupIdentity in *; auto. rewrite Hs1 in HcheckChild. rewrite Hs1. simpl in *.
+          destruct (beqAddr currBlock sh1entryaddrB) eqn:HbeqCBSh1; try(exfalso; congruence).
+          rewrite <-beqAddrFalse in *. rewrite removeDupIdentity; auto.
+        }
+        rewrite HlookupSh1BEq in *. rewrite Hs1 in Hsh1. rewrite Hs1 in HcheckChild. simpl in *.
+        destruct (beqAddr currBlock block) eqn:HbeqBlocks.
+        - rewrite <-beqAddrTrue in HbeqBlocks. subst block. rewrite HlookupCurrBs0. auto.
+        - rewrite <-beqAddrFalse in *. rewrite removeDupIdentity in *; auto.
+      }
+      specialize(Hcons0 block sh1entryaddrB part HbeqBlockBTDP HpartIsPart HblockMapped HcheckChilds0).
+      destruct Hcons0 as (HAflag & HPflag & [startaddr (Hstart & HstartIsPDT)]).
+      (*TODO HERE can we prove that startaddr is not in the range ? If it is, then it is in a shared block, right ?*)
+      assert(HstartNotInRange: ~In startaddr (getAllPaddrBlock startBlock endBlock)).
+      {
+        assert(HnoChild: sh1entryPDchild sh1entryaddrB nullAddr s0).
+        {
+          assert(Hres: PDflagMeansNoChild s0) by (unfold deleteProps in *; intuition).
+          assert(HblockIsBE: isBE block s0).
+          {
+            unfold bentryStartAddr in *. unfold isBE. destruct (lookup block (memory s0) beqAddr); try(congruence).
+            destruct v; try(congruence). trivial.
+          }
+          unfold PDflagMeansNoChild in *. destruct HcheckChilds0 as (HcheckChilds0 & Hsh1). unfold sh1entryAddr in *.
+          unfold checkChild in *.
+          destruct (lookup block (memory s0) beqAddr) eqn:HlookupBlock; try(exfalso; congruence).
+          destruct v; try(exfalso; congruence). subst sh1entryaddrB. apply Hres; trivial. unfold sh1entryPDflag.
+          destruct (lookup (CPaddr (block + sh1offset)) (memory s0) beqAddr); try(congruence). destruct v; congruence.
+        }
+        intro Hcontra. assert(HstartInBlock: In startaddr (getAllPaddrAux [block] s0)).
+        {
+          assert(Hend: exists endaddr, bentryEndAddr block endaddr s0).
+          {
+            unfold bentryEndAddr. unfold bentryStartAddr in *.
+            destruct (lookup block (memory s0) beqAddr); try(exfalso; congruence).
+            destruct v; try(exfalso; congruence). exists (endAddr (blockrange b)). reflexivity.
+          }
+          destruct Hend as [endaddr Hend]. assert(Hwell: wellFormedBlock s0) by (unfold deleteProps in *; intuition).
+          specialize(Hwell block startaddr endaddr HPflag Hstart Hend). destruct Hwell as (Hwell & _). simpl.
+          unfold bentryStartAddr in *. unfold bentryEndAddr in *.
+          destruct (lookup block (memory s0) beqAddr); try(exfalso; congruence). destruct v; try(exfalso; congruence).
+          rewrite app_nil_r. rewrite <-Hstart. rewrite <-Hend. apply IL.getAllPaddrBlockIncl; lia.
+        }
+        assert(HstartInCurr: In startaddr (getMappedPaddr currentPart s0)).
+        {
+          apply IL.addrInBlockIsMapped with currBlock; trivial. rewrite Hranges0. assumption.
+        }
+        assert(Hsh1Val: sh1entryaddrB = CPaddr (block+sh1offset)).
+        {
+          destruct HcheckChilds0 as (_ & Hres). unfold sh1entryAddr in *.
+          destruct (lookup block (memory s0) beqAddr); try(exfalso; congruence). destruct v; try(exfalso; congruence).
+          assumption.
+        }
+        assert(HpartIsAnc: In currentPart (part::filterOptionPaddr (completeParentsList part s0))).
+        {
+          subst sh1entryaddrB. apply addressesBloodlineIfNotSharedPartial with startaddr block blockTDParent
+            blockToDelete; trivial; unfold deleteProps in *; intuition. (*TODO HERE needs more props*)
+(*why is parentOfPartitionIsPartition missing ?*)
+        }
+(*addressesBloodlineIfNotShared addrBelongToAncestors*)
+specialize(HpropsAddrToRemoveCopy startaddr Hcontra).
+      }
+      (*HlookupsEq*)
+      (* END PDTIfPDFlag *)
+    }
+
+    assert(AccessibleNoPDFlag s).
+    { (* BEGIN AccessibleNoPDFlag s *)
+      assert(Hcons0: AccessibleNoPDFlag s0) by (unfold consistency in *; unfold consistency1 in *; intuition).
+      intros block sh1entryaddr HblockIsBE Hsh1 HAflag.
+      
+      
+      
+      
+      (* END AccessibleNoPDFlag *)
+    }
+
+    assert(FirstFreeSlotPointerIsBEAndFreeSlot s).
+    { (* BEGIN FirstFreeSlotPointerIsBEAndFreeSlot s *)
+      assert(Hcons0: FirstFreeSlotPointerIsBEAndFreeSlot s0)
+        by (unfold consistency in *; unfold consistency1 in *; intuition).
+      intros partition pdentry HlookupPart HbeqFirstNull.
+      
+      
+      
+      
+      (* END FirstFreeSlotPointerIsBEAndFreeSlot *)
+    }
+
+    assert(multiplexerIsPDT s).
+    { (* BEGIN multiplexerIsPDT s *)
+      assert(Hcons0: multiplexerIsPDT s0) by (unfold consistency in *; unfold consistency1 in *; intuition).
+      unfold multiplexerIsPDT in *. unfold isPDT in *.
+      
+      
+      
+      
+      (* END multiplexerIsPDT *)
+    }
+
+    assert(currentPartitionInPartitionsList s).
+    { (* BEGIN currentPartitionInPartitionsList s *)
+      assert(Hcons0: currentPartitionInPartitionsList s0)
+        by (unfold consistency in *; unfold consistency1 in *; intuition).
+      
+      
+      
+      
+      
+      (* END currentPartitionInPartitionsList *)
+    }
+
+    assert(wellFormedShadowCutIfBlockEntry s).
+    { (* BEGIN wellFormedShadowCutIfBlockEntry s *)
+      assert(Hcons0: wellFormedShadowCutIfBlockEntry s0)
+        by (unfold consistency in *; unfold consistency1 in *; intuition). intros block HblockIsBE.
+      
+      
+      
+      
+      
+      (* END wellFormedShadowCutIfBlockEntry *)
+    }
+
+    assert(BlocksRangeFromKernelStartIsBE s).
+    { (* BEGIN BlocksRangeFromKernelStartIsBE s *)
+      assert(Hcons0: BlocksRangeFromKernelStartIsBE s0)
+        by (unfold consistency in *; unfold consistency1 in *; intuition).
+      intros kernel idx HkernIsKS HltIdxKernEntries.
+      
+      
+      
+      
+      (* END BlocksRangeFromKernelStartIsBE *)
+    }
+
+    assert(KernelStructureStartFromBlockEntryAddrIsKS s).
+    { (* BEGIN KernelStructureStartFromBlockEntryAddrIsKS s *)
+      assert(Hcons0: KernelStructureStartFromBlockEntryAddrIsKS s0)
+        by (unfold consistency in *; unfold consistency1 in *; intuition). intros block idx HblockIsBE Hidx.
+      
+      
+      
+      
+      
+      (* END KernelStructureStartFromBlockEntryAddrIsKS *)
+    }
+
+    assert(sh1InChildLocationIsBE s).
+    { (* BEGIN sh1InChildLocationIsBE s *)
+      assert(Hcons0: sh1InChildLocationIsBE s0) by (unfold consistency in *; unfold consistency1 in *; intuition).
+      intros sh1entryaddr sh1entry HlookupSh1 HbeqLocNull.
+      
+      
+      
+      
+      (* END sh1InChildLocationIsBE *)
+    }
+
+    assert(StructurePointerIsKS s).
+    { (* BEGIN StructurePointerIsKS s *)
+      assert(Hcons0: StructurePointerIsKS s0) by (unfold consistency in *; unfold consistency1 in *; intuition).
+      intros partition pdentry HlookupPart HbeqStructNull.
+      
+      
+      
+      
+      (* END StructurePointerIsKS *)
+    }
+
+    assert(NextKSIsKS s).
+    { (* BEGIN NextKSIsKS s *)
+      assert(Hcons0: NextKSIsKS s0) by (unfold consistency in *; unfold consistency1 in *; intuition).
+      intros kernel nextKSaddr nextKS HkernIsKS HnextAddr HnextKSAddr HbeqNextNull.
+      
+      
+      
+      
+      (* END NextKSIsKS *)
+    }
+
+    assert(NextKSOffsetIsPADDR s).
+    { (* BEGIN NextKSOffsetIsPADDR s *)
+      assert(Hcons0: NextKSOffsetIsPADDR s0) by (unfold consistency in *; unfold consistency1 in *; intuition).
+      intros kernel nextKSaddr HkernIsKS HnextAddr.
+      
+      
+      
+      
+      (* END NextKSOffsetIsPADDR *)
+    }
+
+    assert(NoDupInFreeSlotsList s).
+    { (* BEGIN NoDupInFreeSlotsList s *)
+      assert(Hcons0: NoDupInFreeSlotsList s0) by (unfold consistency in *; unfold consistency1 in *; intuition).
+      intros partition pdentry HlookupPart.
+      
+      
+      
+      
+      (* END NoDupInFreeSlotsList *)
+    }
+
+    assert(freeSlotsListIsFreeSlot s).
+    { (* BEGIN freeSlotsListIsFreeSlot s *)
+      assert(Hcons0: freeSlotsListIsFreeSlot s0) by (unfold consistency in *; unfold consistency1 in *; intuition).
+      intros partition addr optionfreeslotslist freeslotslist HpartIsPDT HwellFormed HaddrInList HbeqAddrNull.
+      
+      
+      
+      
+      (* END freeSlotsListIsFreeSlot *)
+    }
+
+    assert(DisjointFreeSlotsLists s).
+    { (* BEGIN DisjointFreeSlotsLists s *)
+      assert(Hcons0: DisjointFreeSlotsLists s0) by (unfold consistency in *; unfold consistency1 in *; intuition).
+      intros part1 part2 Hpart1IsPDT Hpart2IsPDT HbeqParts.
+      
+      
+      
+      
+      (* END DisjointFreeSlotsLists *)
+    }
+
+    assert(inclFreeSlotsBlockEntries s).
+    { (* BEGIN inclFreeSlotsBlockEntries s *)
+      assert(Hcons0: inclFreeSlotsBlockEntries s0) by (unfold consistency in *; unfold consistency1 in *; intuition).
+      intros partition HpartIsPDT.
+      
+      
+      
+      
+      (* END inclFreeSlotsBlockEntries *)
+    }
+
+    assert(DisjointKSEntries s).
+    { (* BEGIN DisjointKSEntries s *)
+      assert(Hcons0: DisjointKSEntries s0) by (unfold consistency in *; unfold consistency1 in *; intuition).
+      intros part1 part2 Hpart1IsPDT Hpart2IsPDT HbeqParts.
+      
+      
+      
+      
+      (* END DisjointKSEntries *)
+    }
+
+    assert(noDupPartitionTree s).
+    { (* BEGIN noDupPartitionTree s *)
+      assert(Hcons0: noDupPartitionTree s0) by (unfold consistency in *; unfold consistency1 in *; intuition).
+      
+      
+      
+      
+      
+      (* END noDupPartitionTree *)
+    }
+
+    assert(isParent s).
+    { (* BEGIN isParent s *)
+      assert(Hcons0: isParent s0) by (unfold consistency in *; unfold consistency1 in *; intuition).
+      intros partition pdparent HparentIsPart HpartIsChild.
+      
+      
+      
+      
+      (* END isParent *)
+    }
+
+    assert(isChild s).
+    { (* BEGIN isChild s *)
+      assert(Hcons0: isChild s0) by (unfold consistency in *; unfold consistency1 in *; intuition).
+      intros partition pdparent HpartIsPart HparentIsParent HbeqPartRoot.
+      
+      
+      
+      
+      (* END isChild *)
+    }
+
+    assert(noDupKSEntriesList s).
+    { (* BEGIN noDupKSEntriesList s *)
+      assert(Hcons0: noDupKSEntriesList s0) by (unfold consistency in *; unfold consistency1 in *; intuition).
+      intros partition HpartIsPDT.
+      
+      
+      
+      
+      (* END noDupKSEntriesList *)
+    }
+
+    assert(noDupMappedBlocksList s).
+    { (* BEGIN noDupMappedBlocksList s *)
+      assert(Hcons0: noDupMappedBlocksList s0) by (unfold consistency in *; unfold consistency1 in *; intuition).
+      intros partition HpartIsPDT.
+      
+      
+      
+      
+      (* END noDupMappedBlocksList *)
+    }
+
+    assert(wellFormedBlock s).
+    { (* BEGIN wellFormedBlock s *)
+      assert(Hcons0: wellFormedBlock s0) by (unfold consistency in *; unfold consistency1 in *; intuition).
+      intros block startaddr endaddr HPflag HstartBlock HendBlock.
+      
+      
+      
+      
+      (* END wellFormedBlock *)
+    }
+
+    assert(parentOfPartitionIsPartition s).
+    { (* BEGIN parentOfPartitionIsPartition s *)
+      assert(Hcons0: parentOfPartitionIsPartition s0)
+        by (unfold consistency in *; unfold consistency1 in *; intuition).
+      intros partition pdentry HlookupPart.
+      
+      
+      
+      
+      (* END parentOfPartitionIsPartition *)
+    }
+
+    assert(NbFreeSlotsISNbFreeSlotsInList s).
+    { (* BEGIN NbFreeSlotsISNbFreeSlotsInList s *)
+      assert(Hcons0: NbFreeSlotsISNbFreeSlotsInList s0)
+        by (unfold consistency in *; unfold consistency1 in *; intuition).
+      intros partition nbfreeslots HpartIsPDT HnbFree.
+      
+      
+      
+      
+      (* END NbFreeSlotsISNbFreeSlotsInList *)
+    }
+
+    assert(maxNbPrepareIsMaxNbKernels s).
+    { (* BEGIN maxNbPrepareIsMaxNbKernels s *)
+      assert(Hcons0: maxNbPrepareIsMaxNbKernels s0) by (unfold consistency in *; unfold consistency1 in *; intuition).
+      intros partition kernList HlistOfKerns.
+      
+      
+      
+      
+      (* END maxNbPrepareIsMaxNbKernels *)
+    }
+
+    assert(blockInChildHasAtLeastEquivalentBlockInParent s).
+    { (* BEGIN blockInChildHasAtLeastEquivalentBlockInParent s *)
+      assert(Hcons0: blockInChildHasAtLeastEquivalentBlockInParent s0)
+        by (unfold consistency in *; unfold consistency1 in *; intuition).
+      intros pdparent child block startChild endChild HparentIsPart HchildIsChild HblockMappedChild HstartChild
+        HendChild HPflagChild.
+      
+      
+      
+      
+      (* END blockInChildHasAtLeastEquivalentBlockInParent *)
+    }
+
+    assert(partitionTreeIsTree s).
+    { (* BEGIN partitionTreeIsTree s *)
+      assert(Hcons0: partitionTreeIsTree s0) by (unfold consistency in *; unfold consistency1 in *; intuition).
+      intros child pdparent parentsList HbeqChildRoot HchildIsPart HparentIsParent HparentsList.
+      
+      
+      
+      
+      (* END partitionTreeIsTree *)
+    }
+
+    assert(nextKernelIsValid s).
+    { (* BEGIN nextKernelIsValid s *)
+      assert(Hcons0: nextKernelIsValid s0) by (unfold consistency in *; unfold consistency1 in *; intuition).
+      intros kernel HkernIsKS.
+      
+      
+      
+      
+      (* END nextKernelIsValid *)
+    }
+
+    assert(noDupListOfKerns s).
+    { (* BEGIN noDupListOfKerns s *)
+      assert(Hcons0: noDupListOfKerns s0) by (unfold consistency in *; unfold consistency1 in *; intuition).
+      intros partition kernList HlistOfKerns.
+      
+      
+      
+      
+      (* END noDupListOfKerns *)
+    }
+
+    assert(MPUsizeIsBelowMax s).
+    { (* BEGIN MPUsizeIsBelowMax s *)
+      assert(Hcons0: MPUsizeIsBelowMax s0) by (unfold consistency in *; unfold consistency1 in *; intuition).
+      intros partition MPUlist HMPU.
+      
+      
+      
+      
+      (* END MPUsizeIsBelowMax *)
+    }
+
+    assert(originIsParentBlocksStart s).
+    { (* BEGIN originIsParentBlocksStart s *)
+      assert(Hcons0: originIsParentBlocksStart s0) by (unfold consistency in *; unfold consistency1 in *; intuition).
+      intros partition pdentry block scentryaddr scorigin HpartIsPart HlookupPart HblockMapped Hsce Horigin.
+      
+      
+      
+      
+      (* END originIsParentBlocksStart *)
+    }
+
+    assert(nextImpliesBlockWasCut s).
+    { (* BEGIN nextImpliesBlockWasCut s *)
+      assert(Hcons0: nextImpliesBlockWasCut s0) by (unfold consistency in *; unfold consistency1 in *; intuition).
+      intros partition pdentry block scentryaddr scnext endaddr HpartIsPart HlookupPart HblockMapped HendBlock Hsce
+        HbeqNextNull Hnext HbeqPartRoot.
+      
+      
+      
+      
+      (* END nextImpliesBlockWasCut *)
+    }
+
+    assert(blocksAddressesTypes s).
+    { (* BEGIN blocksAddressesTypes s *)
+      assert(Hcons0: blocksAddressesTypes s0) by (unfold consistency in *; unfold consistency1 in *; intuition).
+      intros block startaddr endaddr HstartBlock HendBlock HPflagBlock HlocBlock.
+      
+      
+      
+      
+      (* END blocksAddressesTypes *)
+    }
+
+    assert(notPDTIfNotPDflag s).
+    { (* BEGIN notPDTIfNotPDflag s *)
+      assert(Hcons0: notPDTIfNotPDflag s0) by (unfold consistency in *; unfold consistency1 in *; intuition).
+      intros block startaddr sh1entryaddr HstartBlock Hsh1 HPflag HPDflag HPDchild.
+      
+      
+      
+      
+      (* END notPDTIfNotPDflag *)
+    }
+
+    assert(nextKernAddrIsInSameBlock s).
+    { (* BEGIN nextKernAddrIsInSameBlock s *)
+      assert(Hcons0: nextKernAddrIsInSameBlock s0) by (unfold consistency in *; unfold consistency1 in *; intuition).
+      intros block kernel startaddr endaddr HstartBlock HendBlock HPflagBlock HPDchildBlock HkernIsKS.
+      
+      
+      
+      
+      (* END nextKernAddrIsInSameBlock *)
+    }
+
+    assert(blockBelongsToAPart s).
+    { (* BEGIN blockBelongsToAPart s *)
+      assert(Hcons0: blockBelongsToAPart s0) by (unfold consistency in *; unfold consistency1 in *; intuition).
+      intros block HPflagBlock.
+      
+      
+      
+      
+      (* END blockBelongsToAPart *)
+    }
+
+    assert(PDflagMeansNoChild s).
+    { (* BEGIN PDflagMeansNoChild s *)
+      assert(Hcons0: PDflagMeansNoChild s0) by (unfold consistency in *; unfold consistency1 in *; intuition).
+      intros block HblockIsBE HPDflagBlock.
+      
+      
+      
+      
+      (* END PDflagMeansNoChild *)
+    }
+
+    assert(nbPrepareIsNbKern s).
+    { (* BEGIN nbPrepareIsNbKern s *)
+      assert(Hcons0: nbPrepareIsNbKern s0) by (unfold consistency in *; unfold consistency1 in *; intuition).
+      intros partition pdentry HlookupPart.
+      
+      
+      
+      
+     (* END nbPrepareIsNbKern *)
+    }
+
+    assert(pdchildIsPDT s).
+    { (* BEGIN pdchildIsPDT s *)
+      assert(Hcons0: pdchildIsPDT s0) by (unfold consistency in *; unfold consistency1 in *; intuition).
+      intros part block sh1entryaddr idchild HpartBisIsPart HblockMapped Hsh1 HPDchild HbeqIdChildNull.
+      
+      
+      
+      
+      (* END pdchildIsPDT *)
+    }
+
+    assert(childBlockNullIfChildNull s).
+    { (* BEGIN childBlockNullIfChildNull s *)
+      assert(Hcons0: childBlockNullIfChildNull s0) by (unfold consistency in *; unfold consistency1 in *; intuition).
+      intros part block sh1entryaddr HpartBisIsPart HblockMapped Hsh1 HPDchild.
+      
+      
+      
+      
+      (* END childBlockNullIfChildNull *)
+    }
+
+    assert(accessibleBlocksArePresent s).
+    { (* BEGIN accessibleBlocksArePresent s *)
+      assert(Hcons0: accessibleBlocksArePresent s0) by (unfold consistency in *; unfold consistency1 in *; intuition).
+      intros block HAflag.
+      
+      
+      
+      
+      (* END accessibleBlocksArePresent *)
+    }
+
+    assert(sharedBlockIsPresent s).
+    { (* BEGIN sharedBlockIsPresent s *)
+      assert(Hcons0: sharedBlockIsPresent s0) by (unfold consistency in *; unfold consistency1 in *; intuition).
+      intros part block child HpartIsPart HblockIsEntry HPDchild HbeqChildNull.
+      
+      
+      
+      
+      (* END sharedBlockIsPresent *)
+    }
+
+    assert(sharedBlockNoPDflagNoLocIsKern s).
+    { (* BEGIN sharedBlockNoPDflagNoLocIsKern s *)
+      assert(Hcons0: sharedBlockNoPDflagNoLocIsKern s0)
+        by (unfold consistency in *; unfold consistency1 in *; intuition).
+      intros part block child startaddr HpartIsPart HblockMapped HPDchild HbeqChildNull HPDflag Hloc Hstart.
+      
+      
+      
+      
+      (* END sharedBlockNoPDflagNoLocIsKern *)
+    }
+
+    assert(partitionNotAutoMapped s).
+    { (* BEGIN partitionNotAutoMapped s *)
+      assert(Hcons0: partitionNotAutoMapped s0) by (unfold consistency in *; unfold consistency1 in *; intuition).
+      intros part HpartIsPart.
+      
+      
+      
+      
+      (* END partitionNotAutoMapped *)
+    }
+
+    assert(configAddrNotMappedInChild s).
+    { (* BEGIN configAddrNotMappedInChild s *)
+      assert(Hcons0: configAddrNotMappedInChild s0) by (unfold consistency in *; unfold consistency1 in *; intuition).
+      intros part child addr HpartIsPart HchildIsChild HaddrIsConfig.
+      
+      
+      
+      (* END configAddrNotMappedInChild *)
+    }
+
+    (* assert(configNotMappedRoot s).
+    { (* BEGIN configNotMappedRoot s *)
+      assert(Hcons0: configNotMappedRoot s0) by (unfold consistency in *; unfold consistency1 in *; intuition).
+      intros addr HaddrIsConfig.
+      
+      
+      
+      (* END configNotMappedRoot *)
+    } *)
+
+    assert(fullKernelIsInOneBlock s).
+    { (* BEGIN fullKernelIsInOneBlock s *)
+      assert(Hcons0: fullKernelIsInOneBlock s0) by (unfold consistency in *; unfold consistency1 in *; intuition).
+      intros part block kernel HpartIsPart HblockMapped HkernInBlock HkernIsKS.
+      
+      
+      
+      (* END fullKernelIsInOneBlock *)
+    }
+
+    assert(sharedBlocksAdressesAreAllMappedInChild s).
+    { (* BEGIN sharedBlocksAdressesAreAllMappedInChild s *)
+      assert(Hcons0: sharedBlocksAdressesAreAllMappedInChild s0)
+        by (unfold consistency in *; unfold consistency1 in *; intuition).
+      intros part block sh1entryaddr blockChild child HpartIsPart HblockMapped Hsh1 HPDchild Hloc HbeqChildNull
+        HbeqLocNull addr HaddrInBlock.
+      
+      
+      
+      (* END sharedBlocksAdressesAreAllMappedInChild *)
+    }
+
+    assert(HpropsAddrToRemoves: forall block startBlock endBlock, In block (getMappedBlocks currentPart s)
+      -> sh1entryPDchild (CPaddr (block+sh1offset)) blockToDelete s
+      -> bentryStartAddr block startBlock s
+      -> bentryEndAddr block endBlock s
+      -> (forall addr, In addr (getAllPaddrBlock startBlock endBlock)
+          -> ~In addr (getPartitions multiplexer s)
+              /\ (forall part, In part (getPartitions multiplexer s)
+                  -> ~In addr (filterOptionPaddr (getKSEntries part s))
+                      /\ ~In addr (getConfigPaddr part s))
+              /\ (isBE addr s -> addr + scoffset < endBlock)
+              /\ (isKS addr s -> addr + nextoffset < endBlock)
+              /\ addr <> nullAddr)).
+    {
+      intros block startaddr endaddr HblockMapped HPDchild Hstart Hend addr HaddrInRange.
+    }
+    (*TODO HERE prove all possible consistency props to see what is left*)
+  }
+  intro isCut. destruct isCut; simpl.
+  + eapply bindRev.
+    { (** Internal.writeAccessibleRec **)
+      eapply weaken. apply ? (*TODO probably needs another lemma*). intros s Hprops. apply Hprops. 
+    }
+    eapply bindRev.
+    { (** indexPredM **)
+      eapply weaken. apply Index.pred. intros s Hprops. apply Hprops. 
+    }
+    intro idxpred. (*apply induction hypothesis*)
+    
+  + eapply bindRev.
+    { (** MALInternal.Index.zero **)
+      eapply weaken. apply Index.zero. intros s Hprops. apply Hprops.
+    }
+    intro zero. destruct (indexEq currIdx zero) eq:HbeqIdxZero.
+    * eapply weaken. apply WP.ret. intros s Hprops. 
+    * eapply bindRev.
+      { (** indexPredM **)
+        eapply weaken. apply Index.pred. intros s Hprops. apply Hprops. 
+      }
+      intro idxpred. (*apply induction hypothesis*)
+- eapply bindRev.
+  { (** MALInternal.Index.zero **)
+    eapply weaken. apply Index.zero. intros s Hprops. apply Hprops.
+  }
+  intro zero. destruct (indexEq currIdx zero) eq:HbeqIdxZero.
+  + eapply weaken. apply WP.ret. intros s Hprops. 
+    
+  + eapply bindRev.
+    { (** indexPredM **)
+      eapply weaken. apply Index.pred. intros s Hprops. apply Hprops. 
+    }
+    intro idxpred. (*apply induction hypothesis*)
+    
+Qed.*)
+
+(*Lemma deleteSharedBlocksRecAux n currentPart kernel blockToDelete:
+{{ fun s => 
+}}
+Internal.deleteSharedBlocksRecAux n currentPart kernel blockToDelete
+{{ fun _ s => 
+}}.
+Proof.
+
+Qed.
+
+Lemma deleteSharedBlocksRec currentPart kernel blockToDelete:
+{{ fun s => 
+}}
+Internal.deleteSharedBlocksRec currentPart kernel blockToDelete
+{{ fun _ s => 
+}}.
+Proof.
+
+Qed.*)
+
+Definition sharedBlockNoPDflagNoLocIsKernModified s :=
+forall part block child startaddr,
+In part (getPartitions multiplexer s)
+-> In block (getMappedBlocks part s)
+-> sh1entryPDchild (CPaddr (block+sh1offset)) child s
+-> child <> nullAddr
+-> sh1entryPDflag (CPaddr (block+sh1offset)) false s
+-> sh1entryInChildLocationWeak (CPaddr (block+sh1offset)) nullAddr s
+-> bentryStartAddr block startaddr s
+-> In startaddr (getConfigBlocks child s)
+    /\ (forall addr child2, In addr (getAllPaddrAux [block] s)
+          -> In child2 (getChildren part s) -> ~In addr (getMappedPaddr child2 s))
+    /\ (forall (addr:paddr) endaddr part2, bentryEndAddr block endaddr s
+          -> In part2 (getPartitions multiplexer s)
+          -> startaddr+Constants.kernelStructureTotalLength <= addr
+          -> addr < endaddr
+          -> ~In addr (getConfigPaddr part2 s)).
+
+Definition configAddrNotMappedInChildModified s :=
+forall part child addr,
+In part (getPartitions multiplexer s)
+-> In child (getChildren part s)
+-> In addr (getConfigPaddr part s)
+-> ~In addr (getUsedPaddr child s).
 
 Lemma deletePartition idPDchildToDelete:
 {{fun s => partitionsIsolation s /\ kernelDataIsolation s /\ verticalSharing s /\ consistency s }}
@@ -163,8 +2098,18 @@ intro eraseSucc. eapply bindRev.
   {
     intros addr HaddrInRange HbeqAddrStart.
     assert(Htypes: blocksAddressesTypes s0) by (unfold consistency in *; unfold consistency1 in *; intuition).
+    assert(Hloc: sh1entryInChildLocationWeak (CPaddr (blockToDeleteInCurrPartAddr + sh1offset)) nullAddr s0).
+    {
+      assert(HnullEquiv: childBlockNullIfChildNull s0)
+        by (unfold consistency in *; unfold consistency1 in *; intuition). destruct HcheckChild as (_ & Hsh1).
+      specialize(HnullEquiv currentPart blockToDeleteInCurrPartAddr (CPaddr (blockToDeleteInCurrPartAddr+sh1offset))
+        HcurrIsParts0 HBTDMapped Hsh1 HPDchild). unfold sh1entryInChildLocation in *.
+      unfold sh1entryInChildLocationWeak.
+      destruct (lookup (CPaddr (blockToDeleteInCurrPartAddr + sh1offset)) (memory s0) beqAddr); try(congruence).
+      destruct v; try(congruence). destruct HnullEquiv. assumption.
+    }
     specialize(Htypes blockToDeleteInCurrPartAddr blockStartAddr blockEndAddr currentPart HcurrIsParts0 HBTDMapped
-      HstartBTDs0 HendBTDs0 HPDchild). destruct Htypes as [(Hcontra & _) | [(_ & Hres) | Hcontra]].
+      HstartBTDs0 HendBTDs0 Hloc). destruct Htypes as [(Hcontra & _) | [(_ & Hres) | Hcontra]].
     - unfold isKS in *. unfold isPDT in *. exfalso.
       destruct (lookup blockStartAddr (memory s0) beqAddr); try(congruence). destruct v; congruence.
     - apply Hres; auto.
@@ -300,6 +2245,8 @@ intro eraseSucc. eapply bindRev.
   assert(HgetAccMappedPEq: forall part, part <> blockStartAddr
     -> getAccessibleMappedPaddr part s = getAccessibleMappedPaddr part s0).
   { intros part HbeqPartStart. apply getAccessibleMappedPaddrEqRemoveAddr with blockStartAddr; trivial. }
+  assert(HgetConfigBEq: forall part, part <> blockStartAddr -> getConfigBlocks part s = getConfigBlocks part s0).
+  { intros part HbeqPartStart. apply getConfigBlocksEqRemoveAddr with blockStartAddr; trivial. }
   assert(HgetConfigEq: forall part, part <> blockStartAddr -> getConfigPaddr part s = getConfigPaddr part s0).
   { intros part HbeqPartStart. apply getConfigPaddrEqRemoveAddr with blockStartAddr; trivial. }
   assert(HgetChildrenEqNotStart: forall part, part <> blockStartAddr -> getChildren part s = getChildren part s0).
@@ -655,16 +2602,6 @@ intro eraseSucc. eapply bindRev.
     assumption.
     (* END partitionTreeIsTree *)
   }
-  assert(kernelEntriesAreValid s).
-  { (* BEGIN kernelEntriesAreValid s *)
-    assert(Hcons0: kernelEntriesAreValid s0) by intuition. intros kernel idx HkernIsKS Hidx. unfold isKS in *.
-    assert(kernel <> blockStartAddr).
-    { intro. subst kernel. rewrite HlookupStarts in *. congruence. }
-    rewrite HlookupsEq in HkernIsKS; trivial. specialize(Hcons0 kernel idx HkernIsKS Hidx). unfold isBE in *.
-    rewrite HlookupsEq; trivial. intro Hcontra. rewrite Hcontra in *. unfold isPDT in *.
-    destruct (lookup blockStartAddr (memory s0) beqAddr); try(congruence). destruct v; congruence.
-    (* END kernelEntriesAreValid *)
-  }
   assert(nextKernelIsValid s).
   { (* BEGIN nextKernelIsValid s *)
     assert(Hcons0: nextKernelIsValid s0) by intuition. intros kernel HkernIsKS. unfold isKS in *.
@@ -777,7 +2714,7 @@ intro eraseSucc. eapply bindRev.
   assert(blocksAddressesTypes s).
   { (* BEGIN blocksAddressesTypes s *)
     assert(Hcons0: blocksAddressesTypes s0) by intuition.
-    intros block startaddr endaddr part HpartIsPart HblockMapped Hstart Hend HPDchildB.
+    intros block startaddr endaddr part HpartIsPart HblockMapped Hstart Hend Hloc.
     apply HgetPartsImpl in HpartIsPart. assert(HbeqPartStart: part <> blockStartAddr).
     {
       intro. subst part. unfold getMappedBlocks in *. unfold getKSEntries in *. rewrite HlookupStarts in *.
@@ -786,10 +2723,10 @@ intro eraseSucc. eapply bindRev.
     rewrite HgetMappedBEq in HblockMapped; trivial. unfold bentryStartAddr in *. assert(block <> blockStartAddr).
     { intro. subst block. rewrite HlookupStarts in *. congruence. }
     unfold bentryEndAddr in *. rewrite HlookupsEq in Hstart; trivial. rewrite HlookupsEq in Hend; trivial.
-    unfold sh1entryPDchild in *. assert(CPaddr (block+sh1offset) <> blockStartAddr).
+    unfold sh1entryInChildLocationWeak in *. assert(CPaddr (block+sh1offset) <> blockStartAddr).
     { intro Hcontra. rewrite Hcontra in *. rewrite HlookupStarts in *. congruence. }
-    rewrite HlookupsEq in HPDchildB; trivial.
-    specialize(Hcons0 block startaddr endaddr part HpartIsPart HblockMapped Hstart Hend HPDchildB).
+    rewrite HlookupsEq in Hloc; trivial.
+    specialize(Hcons0 block startaddr endaddr part HpartIsPart HblockMapped Hstart Hend Hloc).
     destruct Hcons0 as [(HKS & Hrange) | [(HPDT & Hrange) | Hrange]].
     - left. unfold isKS in *. assert(startaddr <> blockStartAddr).
       {
@@ -1221,63 +3158,20 @@ intro eraseSucc. eapply bindRev.
     (* END accessibleBlocksArePresent *)
   }
 
-  assert(isPDT currentPart s).
-  {
-    unfold isPDT. rewrite HlookupsEq; trivial. intro. subst blockStartAddr. unfold getPartitions in *.
-    replace (maxAddr+2) with (S (maxAddr+1)) in HcurrNotInDesc; try(lia). simpl in HcurrNotInDesc.
-    apply Decidable.not_or in HcurrNotInDesc. destruct HcurrNotInDesc. congruence.
-  }
-
-  assert(verticalSharing s).
-  { (* BEGIN verticalSharing s *)
-    intros pdparent child HparentIsPart HchildIsChild. assert(pdparent <> blockStartAddr).
-    { intro. subst pdparent. unfold getChildren in *. rewrite HlookupStarts in *. simpl in *. congruence. }
-    apply HgetPartsImpl in HparentIsPart. apply HgetChildrenImpl in HchildIsChild.
-    rewrite HgetMappedPEq; trivial. specialize(HVSs0 pdparent child HparentIsPart HchildIsChild).
-    unfold getUsedPaddr. intros addr HaddrUsedChild. destruct (beqAddr child blockStartAddr) eqn:HbeqChildStart.
-    - rewrite <-beqAddrTrue in HbeqChildStart. subst child. unfold getConfigPaddr in *. unfold getMappedPaddr in *.
-      unfold getConfigBlocks in *. unfold getMappedBlocks in *. unfold getKSEntries in *. exfalso. simpl in *.
-      rewrite HlookupStarts in *. simpl in *. congruence.
-    - rewrite <-beqAddrFalse in *. rewrite HgetConfigEq in *; trivial. rewrite HgetMappedPEq in *; trivial.
-      apply HVSs0; assumption.
-    (* END verticalSharing *)
-  }
-
-  assert(partitionsIsolation s).
-  { (* BEGIN partitionsIsolation s *)
-    intros pdparent child1 child2 HparentIsPart Hchild1IsChild Hchild2IsChild HbeqChildren.
-    assert(pdparent <> blockStartAddr).
-    { intro. subst pdparent. unfold getChildren in *. rewrite HlookupStarts in *. simpl in *. congruence. }
-    apply HgetPartsImpl in HparentIsPart. apply HgetChildrenImpl in Hchild1IsChild.
-    apply HgetChildrenImpl in Hchild2IsChild.
-    specialize(HPIs0 pdparent child1 child2 HparentIsPart Hchild1IsChild Hchild2IsChild HbeqChildren).
-    unfold getUsedPaddr. destruct (beqAddr child1 blockStartAddr) eqn:HbeqChild1Start.
-    - rewrite <-beqAddrTrue in HbeqChild1Start. subst child1. unfold getConfigPaddr at 1. unfold getMappedPaddr at 1.
-      intros addr HaddrUsed. unfold getConfigBlocks in *. unfold getMappedBlocks in *. unfold getKSEntries in *.
-      simpl in *. rewrite HlookupStarts in *. simpl in *. exfalso; congruence.
-    - destruct (beqAddr child2 blockStartAddr) eqn:HbeqChild2Start.
-      + rewrite <-beqAddrTrue in HbeqChild2Start. subst child2. apply Lib.disjointPermut. unfold getConfigPaddr at 1.
-        unfold getMappedPaddr at 1. intros addr HaddrUsed. unfold getConfigBlocks in *. unfold getMappedBlocks in *.
-        unfold getKSEntries in *. simpl in *. rewrite HlookupStarts in *. simpl in *. exfalso; congruence.
-      + rewrite <-beqAddrFalse in *. rewrite HgetConfigEq; trivial. rewrite HgetMappedPEq; trivial.
-        rewrite HgetConfigEq; trivial. rewrite HgetMappedPEq; trivial.
-    (* END partitionsIsolation *)
-  }
-
-  assert(kernelDataIsolation s).
-  { (* BEGIN kernelDataIsolation s *)
-    intros part1 part2 Hpart1IsPart Hpart2IsPart. apply HgetPartsImpl in Hpart1IsPart.
-    apply HgetPartsImpl in Hpart2IsPart. specialize(HKDIs0 part1 part2 Hpart1IsPart Hpart2IsPart).
-    destruct (beqAddr part1 blockStartAddr) eqn:HbeqPart1Start.
-    - rewrite <-beqAddrTrue in HbeqPart1Start. subst part1. unfold getAccessibleMappedPaddr.
-      unfold getAccessibleMappedBlocks. intros addr HaddrUsed. rewrite HlookupStarts in *. simpl in *.
-      exfalso; congruence.
-    - destruct (beqAddr part2 blockStartAddr) eqn:HbeqPart2Start.
-      + rewrite <-beqAddrTrue in HbeqPart2Start. subst part2. apply Lib.disjointPermut. unfold getConfigPaddr.
-        unfold getMappedPaddr. intros addr HaddrUsed. unfold getConfigBlocks in *. unfold getMappedBlocks in *.
-        unfold getKSEntries in *. simpl in *. rewrite HlookupStarts in *. simpl in *. exfalso; congruence.
-      + rewrite <-beqAddrFalse in *. rewrite HgetConfigEq; trivial. rewrite HgetAccMappedPEq; trivial.
-    (* END kernelDataIsolation *)
+  assert(sharedBlockIsPresent s).
+  { (* BEGIN sharedBlockIsPresent s *)
+    assert(Hcons0: sharedBlockIsPresent s0) by intuition.
+    intros part block child HpartIsPart HblockIsEntry HPDchildB HbeqChildNull. assert(part <> blockStartAddr).
+    {
+      intro. subst part. unfold getKSEntries in *. rewrite HlookupStarts in *. simpl in *. congruence.
+    }
+    apply HgetPartsImpl in HpartIsPart. rewrite HgetKSEq in *; trivial. unfold sh1entryPDchild in *.
+    assert(CPaddr (block + sh1offset) <> blockStartAddr).
+    { intro Hcontra. rewrite Hcontra in *. rewrite HlookupStarts in *. congruence. }
+    rewrite HlookupsEq in HPDchildB; trivial.
+    specialize(Hcons0 part block child HpartIsPart HblockIsEntry HPDchildB HbeqChildNull). unfold bentryPFlag in *.
+    rewrite HlookupsEq; trivial. intro. subst block. rewrite HlookupStart in *. congruence.
+    (* END sharedBlockIsPresent *)
   }
 
   assert(HpartialPDTIfPDFlag: forall idPDchild sh1entryaddr part, idPDchild <> blockToDeleteInCurrPartAddr
@@ -1357,12 +3251,765 @@ intro eraseSucc. eapply bindRev.
     (* END partial PDTIfPDFlag *)
   }
 
+  assert(HstartBTDs: bentryStartAddr blockToDeleteInCurrPartAddr blockStartAddr s).
+  {
+    unfold bentryStartAddr. rewrite HlookupBTDEq. assumption.
+  }
+
+(*TODO HERE prove the modified version*)
+  assert(HpartialSharedNoLocIsKern: forall part block child startaddr,
+    child <> blockStartAddr
+    -> In part (getPartitions multiplexer s)
+    -> In block (getMappedBlocks part s)
+    -> sh1entryPDchild (CPaddr (block + sh1offset)) child s
+    -> child <> nullAddr
+    -> sh1entryPDflag (CPaddr (block + sh1offset)) false s
+    -> sh1entryInChildLocationWeak (CPaddr (block + sh1offset)) nullAddr s
+    -> bentryStartAddr block startaddr s
+    -> In startaddr (getConfigBlocks child s)
+        /\ (forall addr child2, In addr (getAllPaddrAux [block] s)
+              -> In child2 (getChildren part s)
+              -> ~In addr (getMappedPaddr child2 s))
+        /\ (forall (addr:paddr) endaddr part2, bentryEndAddr block endaddr s
+              -> In part2 (getPartitions multiplexer s)
+              -> startaddr+Constants.kernelStructureTotalLength <= addr
+              -> addr < endaddr
+              -> ~In addr (getConfigPaddr part2 s))).
+  { (* BEGIN sharedBlockNoPDflagNoLocIsKern s *)
+    assert(Hcons0: sharedBlockNoPDflagNoLocIsKernModified s0) by (* intuition *) admit.
+    intros part block child startaddr HbeqChildStart HpartIsPart HblockMapped HPDchildB HbeqChildNull HPDflagB Hloc
+      Hstart. assert(part <> blockStartAddr).
+    {
+      intro. subst part. unfold getMappedBlocks in *. unfold getKSEntries in *. rewrite HlookupStarts in *.
+      simpl in *. congruence.
+    }
+    apply HgetPartsImpl in HpartIsPart. rewrite HgetMappedBEq in *; trivial. unfold sh1entryPDchild in *.
+    unfold sh1entryPDflag in *. unfold sh1entryInChildLocationWeak in *. unfold bentryStartAddr in *. simpl.
+    assert(CPaddr (block + sh1offset) <> blockStartAddr).
+    { intro Hcontra. rewrite Hcontra in *. rewrite HlookupStarts in *. congruence. }
+    rewrite HlookupsEq in HPDchildB; trivial. rewrite HlookupsEq in HPDflagB; trivial.
+    rewrite HlookupsEq in Hloc; trivial. assert(block <> blockStartAddr).
+    { intro. subst block. rewrite HlookupStarts in *. congruence. }
+    rewrite HlookupsEq in Hstart; trivial. rewrite HlookupsEq; trivial.
+    specialize(Hcons0 part block child startaddr HpartIsPart HblockMapped HPDchildB HbeqChildNull HPDflagB Hloc
+      Hstart). destruct Hcons0 as (HstartIsConfig & HrangeNotShared & Hunused). rewrite HgetConfigBEq; trivial.
+    split; trivial. split.
+    - intros addr child2 HaddrInBlock Hchild2IsChild. apply HgetChildrenImpl in Hchild2IsChild.
+      specialize(HrangeNotShared addr child2 HaddrInBlock Hchild2IsChild). contradict HrangeNotShared.
+      rewrite <-HgetMappedPEq; trivial. intro. subst child2. unfold getMappedPaddr in *. unfold getMappedBlocks in *.
+      unfold getKSEntries in *. rewrite HlookupStarts in *. simpl in *. congruence.
+    - intros addr endaddr part2 Hend Hpart2IsPart. unfold bentryEndAddr in *. rewrite HlookupsEq in Hend; trivial.
+      assert(part2 <> blockStartAddr).
+      {
+        assert(isPDT part2 s).
+        { apply partitionsArePDTPartial with blockToDeleteInCurrPartAddr blockStartAddr; trivial. }
+      }
+      apply HgetPartsImpl in Hpart2IsPart.
+      HgetConfigEq HlookupStarts
+    (* END sharedBlockNoPDflagNoLocIsKern *)
+  }
+
+  assert(partitionNotAutoMapped s).
+  { (* BEGIN partitionNotAutoMapped s *)
+    assert(Hcons0: partitionNotAutoMapped s0) by intuition. intros part HpartIsPart.
+    apply HgetPartsImpl in HpartIsPart. specialize(Hcons0 part HpartIsPart). contradict Hcons0.
+    rewrite <-HgetMappedPEq; trivial. intro. subst part. unfold getMappedPaddr in *. unfold getMappedBlocks in *.
+    unfold getKSEntries in *. rewrite HlookupStarts in *. simpl in Hcons0. congruence.
+    (* END partitionNotAutoMapped *)
+  }
+
+(*TODO HERE prove the modified version*)
+  assert(configAddrNotMappedInChild s).
+  { (* BEGIN configAddrNotMappedInChild s *)
+    assert(Hcons0: configAddrNotMappedInChild s0) by intuition.
+    intros part child addr HpartIsPart HchildIsChild HaddrIsConfig. assert(part <> blockStartAddr).
+    {
+      intro. subst part. unfold getChildren in *. unfold getMappedBlocks in *. unfold getKSEntries in *.
+      rewrite HlookupStarts in *. simpl in *. congruence.
+    }
+    apply HgetPartsImpl in HpartIsPart. apply HgetChildrenImpl in HchildIsChild. rewrite HgetConfigEq in *; trivial.
+    specialize(Hcons0 part child addr HpartIsPart HchildIsChild HaddrIsConfig). contradict Hcons0.
+    rewrite <-HgetMappedPEq; trivial. intro. subst child. unfold getMappedPaddr in *. unfold getMappedBlocks in *.
+    unfold getKSEntries in *. rewrite HlookupStarts in *. simpl in Hcons0. congruence.
+    (* END configAddrNotMappedInChild *)
+  }
+
+  assert(fullKernelIsInOneBlock s).
+  { (* BEGIN fullKernelIsInOneBlock s *)
+    assert(Hcons0: fullKernelIsInOneBlock s0) by intuition.
+    intros part block kernel HpartIsPart HblockMapped HkernInBlock HkernIsKS. assert(part <> blockStartAddr).
+    {
+      intro. subst part. unfold getMappedBlocks in *. unfold getKSEntries in *. rewrite HlookupStarts in *.
+      simpl in *. congruence.
+    }
+    apply HgetPartsImpl in HpartIsPart. simpl in HkernInBlock. assert(block <> blockStartAddr).
+    { intro. subst block. rewrite HlookupStarts in *. simpl in HkernInBlock. congruence. }
+    rewrite HgetMappedBEq in *; trivial. unfold isKS in *. assert(kernel <> blockStartAddr).
+    { intro. subst kernel. rewrite HlookupStarts in *. congruence. }
+    simpl. rewrite HlookupsEq in HkernInBlock; trivial. rewrite HlookupsEq in HkernIsKS; trivial.
+    rewrite HlookupsEq; trivial.
+    specialize(Hcons0 part block kernel HpartIsPart HblockMapped HkernInBlock HkernIsKS). assumption.
+    (* END fullKernelIsInOneBlock *)
+  }
+
+(*TODO HERE try to prove kernInSameBlock s*)
+
+  assert(HpartialSharedInChild: forall partition block sh1entryaddr blockChild idchild,
+    idchild <> blockStartAddr
+    -> In partition (getPartitions multiplexer s)
+    -> In block (getMappedBlocks partition s)
+    -> sh1entryAddr block sh1entryaddr s
+    -> sh1entryPDchild sh1entryaddr idchild s
+    -> sh1entryInChildLocationWeak sh1entryaddr blockChild s
+    -> idchild <> nullAddr
+    -> blockChild <> nullAddr
+    -> forall addr, In addr (getAllPaddrAux [block] s) -> In addr (getMappedPaddr idchild s)).
+  { (* BEGIN sharedBlocksAdressesAreAllMappedInChild s *)
+    assert(Hcons0: sharedBlocksAdressesAreAllMappedInChild s0) by intuition.
+    intros part block sh1entryaddr blockChild child HbeqChildStart HpartIsPart HblockMapped Hsh1 HPDchildB Hloc
+      HbeqChildNull HbeqLocNull addr HaddrInBlock. assert(part <> blockStartAddr).
+    {
+      intro. subst part. unfold getMappedBlocks in *. unfold getKSEntries in *. rewrite HlookupStarts in *.
+      simpl in *. congruence.
+    }
+    apply HgetPartsImpl in HpartIsPart. unfold sh1entryAddr in *. assert(block <> blockStartAddr).
+    { intro. subst block. rewrite HlookupStarts in *. congruence. }
+    rewrite HgetMappedBEq in *; trivial. simpl in HaddrInBlock. rewrite HlookupsEq in HaddrInBlock; trivial.
+    rewrite HlookupsEq in Hsh1; trivial. unfold sh1entryPDchild in *. unfold sh1entryInChildLocationWeak in *.
+    assert(sh1entryaddr <> blockStartAddr).
+    { intro Hcontra. rewrite Hcontra in *. rewrite HlookupStarts in *. congruence. }
+    rewrite HlookupsEq in HPDchildB; trivial. rewrite HlookupsEq in Hloc; trivial.
+    specialize(Hcons0 part block sh1entryaddr blockChild child HpartIsPart HblockMapped Hsh1 HPDchildB Hloc
+      HbeqChildNull HbeqLocNull addr HaddrInBlock). rewrite HgetMappedPEq; trivial.
+    (* END sharedBlocksAdressesAreAllMappedInChild *)
+  }
+
+  assert(isPDT currentPart s).
+  {
+    unfold isPDT. rewrite HlookupsEq; trivial. intro. subst blockStartAddr. unfold getPartitions in *.
+    replace (maxAddr+2) with (S (maxAddr+1)) in HcurrNotInDesc; try(lia). simpl in HcurrNotInDesc.
+    apply Decidable.not_or in HcurrNotInDesc. destruct HcurrNotInDesc. congruence.
+  }
+
+  assert(verticalSharing s).
+  { (* BEGIN verticalSharing s *)
+    intros pdparent child HparentIsPart HchildIsChild. assert(pdparent <> blockStartAddr).
+    { intro. subst pdparent. unfold getChildren in *. rewrite HlookupStarts in *. simpl in *. congruence. }
+    apply HgetPartsImpl in HparentIsPart. apply HgetChildrenImpl in HchildIsChild.
+    rewrite HgetMappedPEq; trivial. specialize(HVSs0 pdparent child HparentIsPart HchildIsChild).
+    unfold getUsedPaddr. intros addr HaddrUsedChild. destruct (beqAddr child blockStartAddr) eqn:HbeqChildStart.
+    - rewrite <-beqAddrTrue in HbeqChildStart. subst child. unfold getConfigPaddr in *. unfold getMappedPaddr in *.
+      unfold getConfigBlocks in *. unfold getMappedBlocks in *. unfold getKSEntries in *. exfalso. simpl in *.
+      rewrite HlookupStarts in *. simpl in *. congruence.
+    - rewrite <-beqAddrFalse in *. rewrite HgetConfigEq in *; trivial. rewrite HgetMappedPEq in *; trivial.
+      apply HVSs0; assumption.
+    (* END verticalSharing *)
+  }
+
+  assert(partitionsIsolation s).
+  { (* BEGIN partitionsIsolation s *)
+    intros pdparent child1 child2 HparentIsPart Hchild1IsChild Hchild2IsChild HbeqChildren.
+    assert(pdparent <> blockStartAddr).
+    { intro. subst pdparent. unfold getChildren in *. rewrite HlookupStarts in *. simpl in *. congruence. }
+    apply HgetPartsImpl in HparentIsPart. apply HgetChildrenImpl in Hchild1IsChild.
+    apply HgetChildrenImpl in Hchild2IsChild.
+    specialize(HPIs0 pdparent child1 child2 HparentIsPart Hchild1IsChild Hchild2IsChild HbeqChildren).
+    unfold getUsedPaddr. destruct (beqAddr child1 blockStartAddr) eqn:HbeqChild1Start.
+    - rewrite <-beqAddrTrue in HbeqChild1Start. subst child1. unfold getConfigPaddr at 1. unfold getMappedPaddr at 1.
+      intros addr HaddrUsed. unfold getConfigBlocks in *. unfold getMappedBlocks in *. unfold getKSEntries in *.
+      simpl in *. rewrite HlookupStarts in *. simpl in *. exfalso; congruence.
+    - destruct (beqAddr child2 blockStartAddr) eqn:HbeqChild2Start.
+      + rewrite <-beqAddrTrue in HbeqChild2Start. subst child2. apply Lib.disjointPermut. unfold getConfigPaddr at 1.
+        unfold getMappedPaddr at 1. intros addr HaddrUsed. unfold getConfigBlocks in *. unfold getMappedBlocks in *.
+        unfold getKSEntries in *. simpl in *. rewrite HlookupStarts in *. simpl in *. exfalso; congruence.
+      + rewrite <-beqAddrFalse in *. rewrite HgetConfigEq; trivial. rewrite HgetMappedPEq; trivial.
+        rewrite HgetConfigEq; trivial. rewrite HgetMappedPEq; trivial.
+    (* END partitionsIsolation *)
+  }
+
+  assert(kernelDataIsolation s).
+  { (* BEGIN kernelDataIsolation s *)
+    intros part1 part2 Hpart1IsPart Hpart2IsPart. apply HgetPartsImpl in Hpart1IsPart.
+    apply HgetPartsImpl in Hpart2IsPart. specialize(HKDIs0 part1 part2 Hpart1IsPart Hpart2IsPart).
+    destruct (beqAddr part1 blockStartAddr) eqn:HbeqPart1Start.
+    - rewrite <-beqAddrTrue in HbeqPart1Start. subst part1. unfold getAccessibleMappedPaddr.
+      unfold getAccessibleMappedBlocks. intros addr HaddrUsed. rewrite HlookupStarts in *. simpl in *.
+      exfalso; congruence.
+    - destruct (beqAddr part2 blockStartAddr) eqn:HbeqPart2Start.
+      + rewrite <-beqAddrTrue in HbeqPart2Start. subst part2. apply Lib.disjointPermut. unfold getConfigPaddr.
+        unfold getMappedPaddr. intros addr HaddrUsed. unfold getConfigBlocks in *. unfold getMappedBlocks in *.
+        unfold getKSEntries in *. simpl in *. rewrite HlookupStarts in *. simpl in *. exfalso; congruence.
+      + rewrite <-beqAddrFalse in *. rewrite HgetConfigEq; trivial. rewrite HgetAccMappedPEq; trivial.
+    (* END kernelDataIsolation *)
+  }
+
   assert(currentPart <> blockStartAddr).
   {
     contradict HcurrNotInDesc. subst blockStartAddr. unfold getPartitions.
     replace (maxAddr+2) with (S (maxAddr+1)); try(lia). simpl. auto.
   }
+  assert(HbeqStartNull: blockStartAddr <> nullAddr).
+  {
+    assert(isPADDR nullAddr s0) by intuition. intro. subst blockStartAddr. unfold isPADDR in *.
+    rewrite HlookupStart in *. congruence.
+  }
 
+  assert(HnewPartsNotBelowStart: forall part, In part (getPartitions multiplexer s)
+    -> part <> blockStartAddr
+    -> ~In part (getPartitions blockStartAddr s0)).
+  {
+    intros part HpartIsPart HbeqParts. contradict HpartIsPart.
+    apply getPartitionsExcludesRemovedAddr with s0 blockStartAddr; trivial. intuition.
+  }
+
+  assert(HcurrIsPart: In currentPart (getPartitions multiplexer s)).
+  {
+    apply HgetPartsImplRev in HcurrIsParts0. destruct HcurrIsParts0; try(exfalso; congruence). assumption.
+  }
+
+  assert(forall block startBlock endBlock, In block (getMappedBlocks currentPart s)
+    -> sh1entryPDchild (CPaddr (block+sh1offset)) blockStartAddr s
+    -> bentryStartAddr block startBlock s
+    -> bentryEndAddr block endBlock s
+    -> (forall addr, In addr (getAllPaddrBlock startBlock endBlock)
+        -> ~In addr (getPartitions multiplexer s)
+            /\ (forall part, In part (getPartitions multiplexer s)
+                -> ~In addr (filterOptionPaddr (getKSEntries part s))
+                    /\ ~In addr (getConfigPaddr part s))
+            /\ (isBE addr s -> addr + scoffset < endBlock)
+            /\ (isKS addr s -> addr + nextoffset < endBlock)
+            /\ (forall block: paddr, addr = CPaddr (block+sh1offset)
+                  -> In block (getAllPaddrBlock startBlock endBlock))
+            /\ (forall block: paddr, addr = CPaddr (block+scoffset)
+                  -> In block (getAllPaddrBlock startBlock endBlock))
+            /\ addr <> nullAddr)).
+  {
+    intros block startBlock endBlock HblockMapped HPDchildB Hstart Hend addr HaddrInRange.
+    unfold bentryStartAddr in *. assert(block <> blockStartAddr).
+    { intro. subst block. rewrite HlookupStarts in *. congruence. }
+    assert(Hsh1: sh1entryAddr block (CPaddr (block+sh1offset)) s0).
+    {
+      unfold sh1entryAddr. rewrite <-HlookupsEq; trivial. destruct (lookup block (memory s) beqAddr); try(congruence).
+      destruct v; congruence.
+    }
+    rewrite HgetMappedBEq in HblockMapped; trivial.
+    assert(HblockIsEntry: In block (filterOptionPaddr (getKSEntries currentPart s0))).
+    {
+      unfold getMappedBlocks in *. apply InFilterPresentInList in HblockMapped. assumption.
+    }
+    unfold sh1entryPDchild in *. assert(CPaddr (block+sh1offset) <> blockStartAddr).
+    { intro Hcontra. rewrite Hcontra in *. rewrite HlookupStarts in *. congruence. }
+    rewrite HlookupsEq in HPDchildB; trivial.
+    assert(HPDflagB: sh1entryPDflag (CPaddr (block+sh1offset)) false s0).
+    {
+      unfold sh1entryPDflag. unfold sh1entryPDchild in *.
+      destruct (lookup (CPaddr (block+sh1offset)) (memory s0) beqAddr) eqn:HlookupSh1; try(congruence).
+      destruct v; try(congruence). destruct (PDflag s1) eqn:HPD; trivial. exfalso.
+      assert(HPDflagB: sh1entryPDflag (CPaddr (block+sh1offset)) true s0).
+      { unfold sh1entryPDflag. rewrite HlookupSh1. auto. }
+      assert(HchildNull: PDflagMeansNoChild s0) by intuition. assert(HblockIsBE: isBE block s0).
+      {
+        apply IL.mappedBlockIsBE in HblockMapped. destruct HblockMapped as [bentry (Hlookup & _)]. unfold isBE.
+        rewrite Hlookup. trivial.
+      }
+      specialize(HchildNull block HblockIsBE HPDflagB). unfold sh1entryPDchild in *. rewrite HlookupSh1 in *.
+      rewrite <-HchildNull in *. congruence.
+    }
+    rewrite HlookupsEq in Hstart; trivial. unfold bentryEndAddr in *. rewrite HlookupsEq in Hend; trivial.
+    assert(HlocOrConfig: exists blockChild, sh1entryInChildLocationWeak (CPaddr (block+sh1offset)) blockChild s0
+      /\ (blockChild <> nullAddr \/ (In startBlock (getConfigBlocks blockStartAddr s0))
+          /\ (forall addr child2, In addr (getAllPaddrAux [block] s0)
+                -> In child2 (getChildren currentPart s0)
+                -> ~In addr (getMappedPaddr child2 s0))
+          /\ (forall (addr:paddr) endaddr part2, bentryEndAddr block endaddr s0
+                -> In part2 (getPartitions multiplexer s0)
+                -> startBlock+Constants.kernelStructureTotalLength <= addr
+                -> addr < endaddr
+                -> ~In addr (getConfigPaddr part2 s0)))).
+    {
+      unfold sh1entryInChildLocationWeak.
+      destruct (lookup (CPaddr (block+sh1offset)) (memory s0) beqAddr) eqn:HlookupSh1; try(exfalso; congruence).
+      destruct v; try(exfalso; congruence). exists (inChildLocation s1). split; trivial.
+      destruct (beqAddr (inChildLocation s1) nullAddr) eqn:HbeqLocNull.
+      - rewrite <-beqAddrTrue in HbeqLocNull.
+        assert(HPDchildBis: sh1entryPDchild (CPaddr (block+sh1offset)) blockStartAddr s0).
+        { unfold sh1entryPDchild. rewrite HlookupSh1. assumption. }
+        assert(Hloc: sh1entryInChildLocationWeak (CPaddr (block+sh1offset)) nullAddr s0).
+        { unfold sh1entryInChildLocationWeak. rewrite HlookupSh1. auto. }
+        assert(Hres: sharedBlockNoPDflagNoLocIsKernModified s0) by admit(* intuition *).
+        specialize(Hres currentPart block blockStartAddr startBlock). right. apply Hres; trivial.
+      - rewrite <-beqAddrFalse in *. auto.
+    }
+    destruct HlocOrConfig as [blockChild (Hloc & HlocOrConfig)].
+    assert(HaddrMappedStart: blockChild <> nullAddr -> In addr (getMappedPaddr blockStartAddr s0)).
+    {
+      intro HbeqLocNull. assert(Hres: sharedBlocksAdressesAreAllMappedInChild s0) by intuition.
+      assert(HaddrInBlock: In addr (getAllPaddrAux [block] s0)).
+      {
+        simpl. destruct (lookup block (memory s0) beqAddr); try(simpl; congruence).
+        destruct v; try(simpl; congruence). rewrite <-Hstart. rewrite <-Hend. rewrite app_nil_r. assumption.
+      }
+      specialize(Hres currentPart block (CPaddr (block+sh1offset)) blockChild blockStartAddr HcurrIsParts0
+        HblockMapped Hsh1 HPDchildB Hloc HbeqStartNull HbeqLocNull addr HaddrInBlock). assumption.
+    }
+    assert(HconfigIsKS: forall addr part, In addr (getConfigBlocks part s0) -> isKS addr s0).
+    { intros addrB part. apply configBlocksAreKS; intuition. }
+    assert(~In addr (getPartitions multiplexer s)).
+    {
+      intro HaddrIsPart. destruct HlocOrConfig as [HbeqLocNull | HstartIsConfig].
+      - specialize(HaddrMappedStart HbeqLocNull). assert(addr <> blockStartAddr).
+        {
+          intro. subst addr. assert(HpartNotMapped: partitionNotAutoMapped s0) by intuition.
+          specialize(HpartNotMapped blockStartAddr HstartIsParts0). congruence.
+        }
+        assert(HaddrInRemovedParts: In addr (getPartitions blockStartAddr s0)).
+        {
+          apply HgetPartsImpl in HaddrIsPart. apply mappedAddrIsInDescendants; trivial. 1-13: intuition.
+        }
+        apply HnewPartsNotBelowStart in HaddrIsPart; congruence.
+      - destruct HstartIsConfig as (HstartIsConfig & _).
+        assert(HpropsOrAddr: addr = blockStartAddr \/ ~In addr (getPartitions blockStartAddr s0)).
+        {
+          destruct (beqAddr addr blockStartAddr) eqn:HbeqAddrStart; try(rewrite <-beqAddrTrue in *; auto).
+          rewrite <-beqAddrFalse in *. right. apply HnewPartsNotBelowStart; assumption.
+        }
+        apply HgetPartsImpl in HaddrIsPart. apply HconfigIsKS in HstartIsConfig. assert(isPDT addr s0).
+        { apply IL.partitionsArePDT; trivial; intuition. }
+        assert(Htypes: blocksAddressesTypes s0) by intuition. apply HgetPartsImpl in HcurrIsPart.
+        destruct (beqAddr blockChild nullAddr) eqn:HbeqBCNull.
+        + rewrite <-beqAddrTrue in HbeqBCNull. subst blockChild.
+          specialize(Htypes block startBlock endBlock currentPart HcurrIsPart HblockMapped Hstart Hend Hloc).
+          unfold isKS in *. destruct Htypes as [(_ & HlookupRangeB) | [(Hcontra & _) | Hcontra]].
+          * apply HlookupRangeB in HaddrInRange. unfold isPDT in *. unfold isBE in *. unfold isSHE in *.
+            unfold isSCE in *. unfold isPADDR in *. destruct (lookup addr (memory s0) beqAddr); try(congruence).
+            destruct v; try(congruence).
+            destruct HaddrInRange as [Hcontra | [Hcontra | [Hcontra | [Hcontra | Hcontra]]]]; congruence.
+          * unfold isPDT in *. destruct (lookup startBlock (memory s0) beqAddr); try(congruence).
+            destruct v; congruence.
+          * apply Hcontra in HaddrInRange. unfold isPDT in *. rewrite HaddrInRange in *. congruence.
+        + rewrite <-beqAddrFalse in *. specialize(HaddrMappedStart HbeqBCNull).
+          destruct (beqAddr addr blockStartAddr) eqn:HbeqAddrStart.
+          * rewrite <-beqAddrTrue in HbeqAddrStart. subst addr.
+            assert(HaddrInBlock: In blockStartAddr (getAllPaddrAux [block] s0)).
+            {
+              simpl. destruct (lookup block (memory s0) beqAddr); try(simpl; congruence).
+              destruct v; try(simpl; congruence). rewrite <-Hstart. rewrite <-Hend. rewrite app_nil_r. assumption.
+            }
+            assert(block = blockToDeleteInCurrPartAddr).
+            {
+              destruct (beqAddr block blockToDeleteInCurrPartAddr) eqn:HbeqBlocks;
+                try(rewrite beqAddrTrue; assumption). rewrite <-beqAddrFalse in *.
+              assert(HnoDupMappedP: noDupMappedPaddrList s0) by intuition.
+              pose proof (DisjointPaddrInPart currentPart block blockToDeleteInCurrPartAddr blockStartAddr s0
+                HnoDupMappedP HcurrIsPDT HblockMapped HBTDMapped HbeqBlocks HaddrInBlock) as Hcontra. exfalso.
+              contradict Hcontra. simpl. rewrite HlookupBTD in *. rewrite app_nil_r. rewrite <-HstartBTDs0.
+              rewrite <-HendBTDs0. apply IL.getAllPaddrBlockIncl; lia.
+            }
+            subst block. unfold sh1entryPDflag in *.
+            destruct (lookup (CPaddr (blockToDeleteInCurrPartAddr + sh1offset)) (memory s0) beqAddr); try(congruence).
+            destruct v; congruence.
+          * rewrite <-beqAddrFalse in *. destruct HpropsOrAddr as [Hcontra | HaddrNotDesc]; try(congruence).
+            contradict HaddrNotDesc. apply parentsListGivesPartitions; trivial. 1-5: intuition. simpl. right.
+            apply mappedAddrIsInBloodline; trivial; intuition.
+    }
+    assert(forall part, In part (getPartitions multiplexer s)
+      -> ~In addr (filterOptionPaddr (getKSEntries part s)) /\ ~In addr (getConfigPaddr part s)).
+    {
+      intros part HpartIsPart. destruct (beqAddr part blockStartAddr) eqn:HbeqParts.
+      - rewrite <-beqAddrTrue in HbeqParts. subst part. unfold getKSEntries. unfold getConfigPaddr.
+        unfold getConfigBlocks. simpl getAllPaddrPDTAux. rewrite HlookupStarts. simpl. auto.
+      - rewrite <-beqAddrFalse in *. destruct (beqAddr blockChild nullAddr) eqn:HbeqBCNull.
+        + rewrite <-beqAddrTrue in HbeqBCNull. subst blockChild.
+          destruct HlocOrConfig as [Hcontra | (HstartBIsConfig & HrangeNotShared & HdeadAddrs)];
+            try(exfalso; congruence).
+          assert(Hsimpl: ~ In addr (getConfigPaddr part s)
+            -> ~ In addr (filterOptionPaddr (getKSEntries part s)) /\ ~ In addr (getConfigPaddr part s)).
+          {
+            intro HaddrNotConfig. split; trivial. contradict HaddrNotConfig. revert HaddrNotConfig.
+            apply inclKSEntriesConfig; intuition.
+          }
+          apply Hsimpl. rewrite HgetConfigEq; trivial. clear Hsimpl. clear HaddrMappedStart.
+          assert(HaddrInBlock: In addr (getAllPaddrAux [block] s0)).
+          {
+            simpl. destruct (lookup block (memory s0) beqAddr); try(simpl; congruence).
+            destruct v; try(simpl; congruence). rewrite app_nil_r. rewrite <-Hstart. rewrite <-Hend. assumption.
+          }
+          specialize(HrangeNotShared addr blockStartAddr HaddrInBlock HstartIsChilds0). intro HaddrIsConfig.
+          assert(HpartNotDesc: ~In part (getPartitions blockStartAddr s0)).
+          { apply HnewPartsNotBelowStart; trivial. }
+          apply HgetPartsImpl in HpartIsPart.
+          assert(HstartNotAnc: ~In blockStartAddr (filterOptionPaddr (completeParentsList part s0))).
+          {
+            contradict HpartNotDesc. apply parentsListGivesPartitions; trivial. 1-5: intuition.
+            simpl. auto.
+          }
+          assert(HaddrMappedCurr: In addr (getMappedPaddr currentPart s0)).
+          { apply IL.addrInBlockIsMapped with block; trivial. }
+          assert(HpropsOr: In currentPart (part::filterOptionPaddr (completeParentsList part s0))).
+          {
+            apply configAddressesBloodline with addr; trivial; intuition.
+          }
+          specialize(HdeadAddrs addr endBlock part Hend HpartIsPart).
+          assert(HaddrConfigStart: In addr (getConfigPaddr blockStartAddr s0)).
+          {
+            unfold getConfigPaddr. apply in_or_app. right. apply addrInKernIsConfig with startBlock; trivial.
+            - unfold isBE. apply HconfigIsKS in HstartBIsConfig. unfold isKS in *.
+              destruct (lookup startBlock (memory s0) beqAddr); try(congruence).
+              destruct v; try(congruence). trivial.
+            - apply IL.getAllPaddrBlockInclRev in HaddrInRange.
+              destruct HaddrInRange as (HlebStartAddr & HltAddrEnd & _).
+              destruct (Nat.ltb addr (startBlock+Constants.kernelStructureTotalLength)) eqn:HltAddrKernAddr.
+              + apply PeanoNat.Nat.ltb_lt in HltAddrKernAddr. apply IL.getAllPaddrBlockAuxIncl; lia.
+              + apply PeanoNat.Nat.ltb_ge in HltAddrKernAddr. exfalso.
+                specialize(HdeadAddrs HltAddrKernAddr HltAddrEnd). congruence.
+          }
+          simpl in HpropsOr. destruct HpropsOr as [HbeqCurrPart | HcurrIsAnc].
+          * subst part. assert(HconfigNotUsed: configAddrNotMappedInChildModified s0) by admit.
+            specialize(HconfigNotUsed currentPart blockStartAddr addr HcurrIsParts0 HstartIsChilds0 HaddrIsConfig).
+            contradict HconfigNotUsed. unfold getUsedPaddr. apply in_or_app. auto.
+          * assert(Hchild: exists child, pdentryParent child currentPart s0
+              /\ In child (getPartitions multiplexer s0)
+              /\ In child (part::filterOptionPaddr (completeParentsList part s0))).
+            { apply completeParentsListChild; trivial; intuition. }
+            destruct Hchild as [child (Hparent & HchildIsPart & HchildIsAnc)].
+            assert(HchildIsChild: isChild s0) by intuition. assert(HbeqChildRoot: child <> constantRootPartM).
+            {
+              intro Hcontra. assert(HparentOfPart: parentOfPartitionIsPartition s0) by intuition.
+              unfold pdentryParent in *.
+              destruct (lookup child (memory s0) beqAddr) eqn:HlookupChild; try(congruence).
+              destruct v; try(congruence). specialize(HparentOfPart child p0 HlookupChild).
+              destruct HparentOfPart as (_ & HparentOfRoot & _). specialize(HparentOfRoot Hcontra).
+              rewrite HparentOfRoot in *. rewrite Hparent in *.
+              assert(isPADDR nullAddr s0) by intuition. unfold isPDT in *. unfold isPADDR in *.
+              destruct (lookup nullAddr (memory s0) beqAddr); try(congruence). destruct v; congruence.
+            }
+            specialize(HchildIsChild child currentPart HchildIsPart Hparent HbeqChildRoot).
+            assert(HaddrUsedChild: In addr (getUsedPaddr child s0)).
+            {
+              simpl in HchildIsAnc. unfold getUsedPaddr. apply in_or_app.
+              destruct HchildIsAnc as [Heq | HchildIsAnc]; try(subst child; left; assumption). right.
+              assert(HparentPart: exists pdparent,
+                In child (pdparent::filterOptionPaddr (completeParentsList pdparent s0))
+                /\ In pdparent (getPartitions multiplexer s0)
+                /\ In addr (getMappedPaddr pdparent s0)).
+              {
+                unfold completeParentsList in HchildIsAnc. set(succ:= S maxAddr). fold succ in HchildIsAnc.
+                cbn -[succ] in HchildIsAnc. destruct (lookup part (memory s0) beqAddr) eqn:HlookupPart;
+                  try(simpl in HchildIsAnc; exfalso; congruence).
+                destruct v; try(simpl in HchildIsAnc; exfalso; congruence).
+                destruct (beqAddr part constantRootPartM) eqn:HbeqPartRoot; cbn -[succ] in HchildIsAnc;
+                  try(exfalso; congruence). exists (parent p0).
+                assert(HparentOfPart: parentOfPartitionIsPartition s0) by intuition.
+                specialize(HparentOfPart part p0 HlookupPart). destruct HparentOfPart as (HparentIsPart & _).
+                rewrite <-beqAddrFalse in *. specialize(HparentIsPart HbeqPartRoot).
+                destruct HparentIsPart as (_ & HparentIsPart). split; try(split); trivial.
+                - simpl. destruct HchildIsAnc as [Heq | HchildIsAnc]; auto. right. unfold completeParentsList.
+                  apply completeParentsListRecN with succ; trivial; lia.
+                - unfold verticalSharing in *. unfold incl in *. apply HVSs0 with part; trivial.
+                  + assert(Hres: isChild s0) by intuition. apply Hres; trivial. unfold pdentryParent.
+                    rewrite HlookupPart. reflexivity.
+                  + unfold getUsedPaddr. apply in_or_app. auto.
+              }
+              destruct HparentPart as [pdparent (HchildIsAncRec & HparentIsPart & HaddrMappedParent)].
+              simpl in HchildIsAncRec. destruct HchildIsAncRec as [Heq | HchildIsAncRec];
+                try(subst child; assumption). assert(childPaddrIsIntoParent s0).
+              { apply IL.blockInclImpliesAddrIncl; intuition. }
+              apply addrBelongToAncestors with pdparent; trivial; intuition.
+            }
+            assert(In addr (getAllPaddrBlockAux 0 startBlock Constants.kernelStructureTotalLength)).
+            {
+              apply IL.getAllPaddrBlockInclRev in HaddrInRange.
+              destruct HaddrInRange as (HlebStartAddr & HltAddrEnd & _).
+              destruct (Nat.ltb addr (startBlock+Constants.kernelStructureTotalLength)) eqn:HltAddrKernAddr.
+              - apply PeanoNat.Nat.ltb_lt in HltAddrKernAddr. apply IL.getAllPaddrBlockAuxIncl; lia.
+              - apply PeanoNat.Nat.ltb_ge in HltAddrKernAddr. exfalso.
+                specialize(HdeadAddrs HltAddrKernAddr HltAddrEnd). congruence.
+            }
+            assert(child = blockStartAddr).
+            {
+              destruct (beqAddr child blockStartAddr) eqn:HbeqChildStart; try(rewrite beqAddrTrue; assumption).
+              exfalso. rewrite <-beqAddrFalse in *.
+              specialize(HPIs0 currentPart child blockStartAddr HcurrIsParts0 HchildIsChild HstartIsChilds0
+                HbeqChildStart addr HaddrUsedChild). contradict HPIs0. unfold getUsedPaddr. apply in_or_app.
+              left. unfold getConfigPaddr. apply in_or_app. right.
+              apply addrInKernIsConfig with startBlock; try(assumption).
+              unfold isBE. apply HconfigIsKS in HstartBIsConfig. unfold isKS in *.
+              destruct (lookup startBlock (memory s0) beqAddr); try(congruence).
+              destruct v; try(congruence). trivial.
+            }
+            subst child. simpl in HchildIsAnc. destruct HchildIsAnc; congruence.
+        + rewrite <-beqAddrFalse in *. specialize(HaddrMappedStart HbeqBCNull).
+          assert(HpartNotInDescStart: ~In part (getPartitions blockStartAddr s0)).
+          { apply HnewPartsNotBelowStart; trivial. }
+          apply HgetPartsImpl in HpartIsPart. rewrite HgetKSEq; trivial. rewrite HgetConfigEq; trivial.
+          apply Decidable.not_or. intro HaddrIn.
+          assert(HaddrInConfig: In addr (getConfigPaddr part s0)).
+          { destruct HaddrIn; trivial. apply inclKSEntriesConfig; trivial; intuition. }
+          clear HaddrIn. assert(HaddrMappedInAllAnc: forall partAnc,
+            In partAnc (filterOptionPaddr (completeParentsList blockStartAddr s0))
+            -> In addr (getMappedPaddr partAnc s0)).
+          {
+            intros partAnc HpartAncIsAncStart.
+            assert(HpartAncIsPart: In partAnc (getPartitions multiplexer s0)).
+            {
+              apply IL.partInParentsListIsPartition with (filterOptionPaddr (completeParentsList blockStartAddr s0))
+                blockStartAddr; trivial.
+              - intuition.
+              - apply completeParentsListIsParentsList; trivial. intuition.
+            }
+            revert HpartAncIsAncStart HaddrMappedStart. apply addrBelongToAncestors; trivial.
+            1-5: intuition. apply IL.blockInclImpliesAddrIncl; intuition.
+          }
+          assert(HaddrMappedMult: In addr (getMappedPaddr multiplexer s0)).
+          {
+            destruct (beqAddr multiplexer blockStartAddr) eqn:HbeqMultStart.
+            - rewrite <-beqAddrTrue in HbeqMultStart. subst blockStartAddr. assumption.
+            - rewrite <-beqAddrFalse in *. apply HaddrMappedInAllAnc.
+              apply getPartitionsGivesAncestor with (maxAddr+2); trivial. 1-7: intuition.
+              unfold getPartitions. replace (maxAddr+2) with (S (maxAddr+1)); try(lia). simpl. auto.
+          }
+          assert(HpropsOr: In part (filterOptionPaddr (completeParentsList blockStartAddr s0))
+              \/ ~In part (filterOptionPaddr (completeParentsList blockStartAddr s0)))
+            by (apply Classical_Prop.classic).
+          assert(isPDT part s0) by (apply IL.partitionsArePDT; trivial; intuition).
+          assert(HaddrInUsed: In addr (getUsedPaddr part s0)).
+          { unfold getUsedPaddr. apply in_or_app. auto. }
+          destruct HpropsOr as [HpartIsAnc | HpartNotAnc].
+          * (* apply HaddrMappedInAllAnc in HpartIsAnc. *)
+            assert(Hchild: exists child, In child (getChildren part s0) /\ In addr (getMappedPaddr child s0)).
+            {
+              assert(Hres: exists child, pdentryParent child part s0
+                 /\ In child (getPartitions multiplexer s0)
+                 /\ In child (blockStartAddr :: filterOptionPaddr (completeParentsList blockStartAddr s0))).
+              {
+                apply completeParentsListChild; trivial; intuition.
+              }
+              destruct Hres as [child (Hparent & HchildIsPart & HchildIsAnc)]. exists child.
+              assert(HisChild: isChild s0) by intuition. assert(HbeqChildRoot: child <> constantRootPartM).
+              {
+                intro Hcontra. unfold pdentryParent in *.
+                destruct (lookup child (memory s0) beqAddr) eqn:HlookupChild; try(congruence).
+                destruct v; try(congruence). assert(HparentOfPart: parentOfPartitionIsPartition s0) by intuition.
+                specialize(HparentOfPart child p0 HlookupChild). destruct HparentOfPart as (_ & HparentOfRoot & _).
+                specialize(HparentOfRoot Hcontra). rewrite HparentOfRoot in *.
+                subst part. assert(isPADDR nullAddr s0) by intuition. unfold isPDT in *. unfold isPADDR in *.
+                destruct (lookup nullAddr (memory s0) beqAddr); try(congruence). destruct v; congruence.
+              }
+              specialize(HisChild child part HchildIsPart Hparent HbeqChildRoot). split; trivial. simpl in *.
+              destruct HchildIsAnc as [HbeqStartChild | HchildIsAnc].
+              - subst child. assumption.
+              - apply HaddrMappedInAllAnc; assumption.
+            }
+            destruct Hchild as [child (HchildIsChild & HaddrMappedChild)].
+            assert(Hres: configAddrNotMappedInChild s0) by intuition.
+            specialize(Hres part child addr HpartIsPart HchildIsChild HaddrInConfig). congruence.
+          * assert(HbeqPartRoot: part <> constantRootPartM).
+            {
+              intro. subst part. contradict HpartNotAnc. unfold multiplexer in HstartIsParts0.
+              apply getPartitionsGivesAncestor with (maxAddr+2); trivial; intuition.
+            }
+            unfold isPDT in *. destruct (lookup part (memory s0) beqAddr) eqn:HlookupPart; try(congruence).
+            destruct v; try(congruence). assert(HparentOfPart: parentOfPartitionIsPartition s0) by intuition.
+            specialize(HparentOfPart part p0 HlookupPart). destruct HparentOfPart as (HparentIsPart & _).
+            specialize(HparentIsPart HbeqPartRoot).
+            destruct HparentIsPart as ([parentEntry HlookupParent] & HparentIsPart).
+            assert(HpartIsChild: isChild s0) by intuition. assert(Hparent: pdentryParent part (parent p0) s0).
+            { unfold pdentryParent. rewrite HlookupPart. reflexivity. }
+            specialize(HpartIsChild part (parent p0) HpartIsPart Hparent HbeqPartRoot).
+            specialize(HVSs0 (parent p0) part HparentIsPart HpartIsChild addr HaddrInUsed).
+            assert(HparentIsAnc: In (parent p0) (filterOptionPaddr (completeParentsList blockStartAddr s0))).
+            {
+              assert(HbeqParentStart: blockStartAddr <> parent p0).
+              {
+                intro Hcontra. rewrite <-Hcontra in *. unfold getPartitions in HpartNotInDescStart.
+                replace (maxAddr+2) with (S (maxAddr+1)) in HpartNotInDescStart; try(lia). simpl in *.
+                apply Decidable.not_or in HpartNotInDescStart.
+                destruct HpartNotInDescStart as (_ & HpartNotDescStart).
+                contradict HpartNotDescStart. induction (getChildren blockStartAddr s0); simpl in *; try(congruence).
+                destruct HpartIsChild as [Heq | HpartIsChild];
+                  try(subst a; rewrite PeanoNat.Nat.add_1_r; simpl; auto).
+                apply in_or_app. auto.
+              }
+              assert(Hbloodline: In (parent p0) (filterOptionPaddr (completeParentsList blockStartAddr s0))
+                \/ parent p0 = blockStartAddr
+                \/ In blockStartAddr (filterOptionPaddr (completeParentsList (parent p0) s0))).
+              {
+                apply addressesBloodline with addr; trivial; intuition.
+              }
+              destruct Hbloodline as [Hres | [Hcontra | Hcontra]]; trivial; exfalso; try(congruence).
+              assert(HcontraPart: In blockStartAddr (part::filterOptionPaddr (completeParentsList part s0))).
+              {
+                assert(HisParentsList: isParentsList s0 (filterOptionPaddr (completeParentsList (parent p0) s0))
+                  (parent p0)).
+                { apply completeParentsListIsParentsList. intuition. unfold isPDT; rewrite HlookupParent; trivial. }
+                assert(HnoDupList: NoDup (filterOptionPaddr (completeParentsList (parent p0) s0))).
+                { revert HisParentsList. apply IL.parentOfPartNotInParentsListsTail; intuition. }
+                apply IL.lengthNoDupPartitions in HnoDupList. simpl. right.
+                unfold completeParentsList in *. replace (S maxAddr) with (maxAddr+1); try(lia). simpl.
+                rewrite HlookupPart. rewrite beqAddrFalse in *. rewrite HbeqPartRoot. simpl. right.
+                assert(Hleb: maxAddr+1 <= S (S maxAddr)) by lia.
+                pose proof (completeParentsListRecEqIfLenLowEnough (parent p0) s0 (maxAddr+1) (S (S maxAddr)) Hleb
+                  HnoDupList) as Heq. rewrite Heq. assumption.
+              }
+              contradict HpartNotInDescStart. revert HcontraPart.
+              apply parentsListGivesPartitions; trivial; intuition.
+            }
+            assert(HotherChild: exists child, pdentryParent child (parent p0) s0
+              /\ In child (getPartitions multiplexer s0)
+              /\ In child (blockStartAddr :: filterOptionPaddr (completeParentsList blockStartAddr s0))).
+            {
+              apply completeParentsListChild; trivial; intuition.
+            }
+            destruct HotherChild as [child (HparentOther & HchildIsPart & HchildIsAnc)].
+            assert(HchildIsChild: isChild s0) by intuition. assert(HbeqChildRoot: child <> constantRootPartM).
+            {
+              unfold pdentryParent in *.
+              destruct (lookup child (memory s0) beqAddr) eqn:HlookupChild; try(exfalso; congruence).
+              destruct v; try(exfalso; congruence).
+              assert(HparentOfPart: parentOfPartitionIsPartition s0) by intuition.
+              specialize(HparentOfPart child p1 HlookupChild). destruct HparentOfPart as (_ & HparentOfRoot & _).
+              intro Hcontra. specialize(HparentOfRoot Hcontra). rewrite HparentOfRoot in *. rewrite HparentOther in *.
+              assert(isPADDR nullAddr s0) by intuition. unfold isPADDR in *. rewrite HlookupParent in *. congruence.
+            }
+            specialize(HchildIsChild child (parent p0) HchildIsPart HparentOther HbeqChildRoot).
+            assert(HbeqPartChild: part <> child).
+            {
+              intro. subst child. simpl in *. destruct HchildIsAnc; congruence.
+            }
+            specialize(HPIs0 (parent p0) part child HparentIsPart HpartIsChild HchildIsChild HbeqPartChild addr
+              HaddrInUsed). unfold getUsedPaddr in *. apply Lib.in_app_or_neg in HPIs0.
+            destruct HPIs0 as (_ & Hcontra).
+            contradict Hcontra. simpl in *. destruct HchildIsAnc as [Heq | HchildIsAnc]; try(subst child; assumption).
+            apply HaddrMappedInAllAnc; assumption.
+    }
+
+    assert(isBE addr s -> addr + scoffset < endBlock).
+    {
+      intro HaddrIsBE. assert(Hkern: KernelStructureStartFromBlockEntryAddrIsKS s) by intuition.
+      assert(Hblkidx: exists idx, bentryBlockIndex addr idx s).
+      {
+        unfold bentryBlockIndex. unfold isBE in *.
+        destruct (lookup addr (memory s) beqAddr); try(exfalso; congruence). destruct v; try(exfalso; congruence).
+        exists (blockindex b0). reflexivity.
+      }
+      destruct Hblkidx as [idx Hblkidx]. specialize(Hkern addr idx HaddrIsBE Hblkidx). unfold bentryBlockIndex in *.
+      destruct (lookup addr (memory s) beqAddr) eqn:HlookupAddr; try(exfalso; congruence).
+      destruct v; try(exfalso; congruence).
+      assert(idx < kernelStructureEntriesNb) by (rewrite Hblkidx; apply Hidx).
+      assert(addr-idx+nextoffset < endBlock).
+      {
+        assert(Hres: fullKernelIsInOneBlock s0) by intuition.
+        assert(HkernInBlock: In (CPaddr (addr-idx)) (getAllPaddrAux [block] s0)).
+        {
+          assert(HresB: kernInSameBlock s0) by admit. unfold kernInSameBlock in *.
+          apply HresB with currentPart; trivial.
+          - simpl. destruct (lookup block (memory s0) beqAddr); try(simpl; congruence).
+            destruct v; try(simpl; congruence). rewrite <-Hstart. rewrite <-Hend. rewrite app_nil_r. assumption.
+          - unfold bentryBlockIndex. assert(~ In addr (getAllPaddrBlock blockStartAddr blockEndAddr)).
+            {
+              intro Hcontra. apply HlookupRange in Hcontra. congruence.
+            }
+            rewrite <-HlookupNotRange; trivial. rewrite HlookupAddr. assumption.
+        }
+        assert(Hkerns0: isKS (CPaddr (addr-idx)) s0).
+        {
+          unfold isKS in *. rewrite <-HlookupNotRange; trivial. intro Hcontra. apply HlookupRange in Hcontra.
+          rewrite Hcontra in *. congruence.
+        }
+        specialize(Hres currentPart block (CPaddr (addr-idx)) HcurrIsParts0 HblockMapped HkernInBlock Hkerns0).
+        assert(HkernEq: ADT.p (CPaddr (addr-idx)) = addr-idx).
+        {
+          unfold CPaddr. assert(addr <= maxAddr) by (apply Hp).
+          destruct (Compare_dec.le_dec (addr - idx) maxAddr); try(lia). reflexivity.
+        }
+        rewrite HkernEq in Hres. destruct Hres as (HlebNextMax & Hres). unfold CPaddr in Hres.
+        destruct (Compare_dec.le_dec (addr - idx + nextoffset) maxAddr); try(lia). simpl in Hres.
+        destruct (lookup block (memory s0) beqAddr); try(exfalso; congruence).
+        destruct v; try(exfalso; congruence). rewrite <-Hstart in *. rewrite <-Hend in *. rewrite app_nil_r in *.
+        apply IL.getAllPaddrBlockInclRev in Hres. simpl in Hres. apply Hres.
+      }
+      rewrite scoffsetVal. rewrite nextoffsetVal in *. lia.
+    }
+
+    assert(isKS addr s -> addr + nextoffset < endBlock).
+    {
+      intro HaddrIsKS. assert(Hres: fullKernelIsInOneBlock s) by assumption.
+      rewrite <-HgetMappedBEq in HblockMapped; trivial. rewrite <-HlookupsEq in Hstart; trivial.
+      rewrite <-HlookupsEq in Hend; trivial. assert(HaddrInBlock: In addr (getAllPaddrAux [block] s)).
+      {
+        simpl. destruct (lookup block (memory s) beqAddr); try(simpl; congruence).
+        destruct v; try(simpl; congruence). rewrite <-Hstart. rewrite <-Hend. rewrite app_nil_r. assumption.
+      }
+      specialize(Hres currentPart block addr HcurrIsPart HblockMapped HaddrInBlock HaddrIsKS).
+      destruct Hres as (HlebNextMax & Hres). unfold CPaddr in Hres.
+      destruct (Compare_dec.le_dec (addr + nextoffset) maxAddr); try(lia). simpl in Hres.
+      destruct (lookup block (memory s) beqAddr); try(exfalso; congruence).
+      destruct v; try(exfalso; congruence). rewrite <-Hstart in *. rewrite <-Hend in *. rewrite app_nil_r in *.
+      apply IL.getAllPaddrBlockInclRev in Hres. simpl in Hres. apply Hres.
+    }
+
+    assert(addr <> nullAddr).
+    {
+      intro Hcontra. destruct (beqAddr addr startBlock) eqn:HbeqAddrStartB.
+      - rewrite <-beqAddrTrue in HbeqAddrStartB. subst addr. subst startBlock.
+        assert(HlastDesc: exists desc blockDesc, In desc (getPartitions multiplexer s0)
+          /\ In blockDesc (getMappedBlocks desc s0) /\ bentryStartAddr blockDesc nullAddr s0
+          /\ sh1entryInChildLocationWeak (CPaddr (blockDesc+sh1offset)) nullAddr s0).
+        {
+          apply lastDescendantBlock with currentPart block; trivial; intuition.
+        }
+        destruct HlastDesc as [desc [blockDesc (HdescIsPart & HBDMapped & HstartBD & HlocBD)]].
+        assert(Htypes: blocksAddressesTypes s0) by intuition.
+        assert(HendBD: exists endBD, bentryEndAddr blockDesc endBD s0).
+        {
+          unfold bentryEndAddr. unfold bentryStartAddr in *.
+          destruct (lookup blockDesc (memory s0) beqAddr); try(exfalso; congruence).
+          destruct v; try(exfalso; congruence). exists (endAddr (blockrange b0)). reflexivity.
+        }
+        destruct HendBD as [endBD HendBD].
+        specialize(Htypes blockDesc nullAddr endBD desc HdescIsPart HBDMapped HstartBD HendBD HlocBD).
+        assert(Hnull: isPADDR nullAddr s0) by intuition. unfold isPADDR in *.
+        destruct Htypes as [(HKS & _) | [(HPDT & _) | Hnone]].
+        + unfold isKS in *. destruct (lookup nullAddr (memory s0) beqAddr); try(congruence). destruct v; congruence.
+        + unfold isPDT in *. destruct (lookup nullAddr (memory s0) beqAddr); try(congruence). destruct v; congruence.
+        + assert(HnullInBlock: In nullAddr (getAllPaddrBlock nullAddr endBD)).
+          {
+            assert(HPflagBD: bentryPFlag blockDesc true s0).
+            {
+              apply IL.mappedBlockIsBE in HBDMapped. destruct HBDMapped as [bentry (Hlookup & Hpres)].
+              unfold bentryPFlag. rewrite Hlookup. auto.
+            }
+            assert(HwellBD: wellFormedBlock s0) by intuition.
+            specialize(HwellBD blockDesc nullAddr endBD HPflagBD HstartBD HendBD). destruct HwellBD as (HwellBD & _).
+            apply IL.getAllPaddrBlockIncl; lia.
+          }
+          apply Hnone in HnullInBlock. rewrite HnullInBlock in *. congruence.
+      - rewrite <-beqAddrFalse in *. subst addr. apply paddrNeqNatNeqEquiv in HbeqAddrStartB.
+        cbn in HbeqAddrStartB. apply IL.getAllPaddrBlockInclRev in HaddrInRange. cbn in HaddrInRange.
+        destruct HaddrInRange as (Hcontra & _). lia.
+    }
+
+    assert(Hrange: getAllPaddrAux [block] s0 = getAllPaddrBlock startBlock endBlock).
+    {
+      simpl. destruct (lookup block (memory s0) beqAddr); try(exfalso; congruence).
+      destruct v; try(exfalso; congruence). rewrite <-Hstart. rewrite <-Hend. apply app_nil_r.
+    }
+
+    assert(forall block: paddr, addr = CPaddr (block+sh1offset) -> In block (getAllPaddrBlock startBlock endBlock)).
+    {
+      intros blockB HaddrEq. subst addr. rewrite <-Hrange in *.
+    }
+
+    assert(forall block: paddr, addr = CPaddr (block+scoffset) -> In block (getAllPaddrBlock startBlock endBlock)).
+    {
+      intros blockB HaddrEq. subst addr. rewrite <-Hrange in *.
+    }
+    auto.
+  }
+
+(*TODO HERE modify the propagated consistency props:
+  partial sharedBlockNoPDflagNoLocIsKern modified
+  kernInSameBlock added*)
   instantiate(1 := fun s => blockToDeleteInCurrPartAddr = idPDchildToDelete
     /\ isBE blockToDeleteInCurrPartAddr s
     /\ bentryStartAddr blockToDeleteInCurrPartAddr blockStartAddr s
@@ -1399,11 +4046,38 @@ intro eraseSucc. eapply bindRev.
           -> In partition (getChildren pdparent s) -> pdentryParent partition pdparent s)
     /\ isChild s /\ noDupKSEntriesList s /\ noDupMappedBlocksList s /\ wellFormedBlock s
     /\ NbFreeSlotsISNbFreeSlotsInList s /\ maxNbPrepareIsMaxNbKernels s
-    /\ blockInChildHasAtLeastEquivalentBlockInParent s /\ partitionTreeIsTree s /\ kernelEntriesAreValid s
+    /\ blockInChildHasAtLeastEquivalentBlockInParent s /\ partitionTreeIsTree s
     /\ nextKernelIsValid s /\ noDupListOfKerns s /\ MPUsizeIsBelowMax s /\ originIsParentBlocksStart s
     /\ nextImpliesBlockWasCut s /\ blocksAddressesTypes s /\ notPDTIfNotPDflag s /\ nextKernAddrIsInSameBlock s
     /\ PDflagMeansNoChild s /\ nbPrepareIsNbKern s /\ pdchildIsPDT s /\ childBlockNullIfChildNull s
-    /\ accessibleBlocksArePresent s /\ noDupMappedPaddrList s /\ accessibleParentPaddrIsAccessibleIntoChild s
+    /\ accessibleBlocksArePresent s /\ sharedBlockIsPresent s
+    /\ (*partial sharedBlockNoPDflagNoLocIsKern*)
+        (forall part block child startaddr,
+          child <> blockStartAddr
+          -> In part (getPartitions multiplexer s)
+          -> In block (getMappedBlocks part s)
+          -> sh1entryPDchild (CPaddr (block + sh1offset)) child s
+          -> child <> nullAddr
+          -> sh1entryPDflag (CPaddr (block + sh1offset)) false s
+          -> sh1entryInChildLocationWeak (CPaddr (block + sh1offset)) nullAddr s
+          -> bentryStartAddr block startaddr s
+          -> In startaddr (getConfigBlocks child s)
+              /\ (forall addr child2, In addr (getAllPaddrAux [block] s)
+                    -> In child2 (getChildren part s)
+                    -> ~In addr (getMappedPaddr child2 s)))
+    /\ partitionNotAutoMapped s /\ configAddrNotMappedInChild s /\ fullKernelIsInOneBlock s
+    /\ (*partial sharedBlocksAdressesAreAllMappedInChild*)
+        (forall partition block sh1entryaddr blockChild idchild,
+          idchild <> blockStartAddr
+          -> In partition (getPartitions multiplexer s)
+          -> In block (getMappedBlocks partition s)
+          -> sh1entryAddr block sh1entryaddr s
+          -> sh1entryPDchild sh1entryaddr idchild s
+          -> sh1entryInChildLocationWeak sh1entryaddr blockChild s
+          -> idchild <> nullAddr
+          -> blockChild <> nullAddr
+          -> forall addr, In addr (getAllPaddrAux [block] s) -> In addr (getMappedPaddr idchild s))
+    /\ noDupMappedPaddrList s /\ accessibleParentPaddrIsAccessibleIntoChild s
     /\ sharedBlockPointsToChild s /\ adressesRangePreservedIfOriginAndNextOk s /\ childsBlocksPropsInParent s
     /\ noChildImpliesAddressesNotShared s /\ kernelsAreNotAccessible s /\ blockAndNextAreSideBySide s
     /\ parentBlocksBoundsIfNoNext s
@@ -1433,6 +4107,19 @@ intro eraseSucc. eapply bindRev.
           -> (forall startaddr, bentryStartAddr block startaddr s -> bentryStartAddr blockChild startaddr s)
                 /\ In blockChild (getMappedBlocks idchild s))
     /\ partitionsIsolation s /\ kernelDataIsolation s /\ verticalSharing s
+    /\ (*partial sharedBlockNoPDflagNoLocIsKern*)
+        (forall block startBlock endBlock, In block (getMappedBlocks currentPart s)
+          -> sh1entryPDchild (CPaddr (block+sh1offset)) blockStartAddr s
+          -> bentryStartAddr block startBlock s
+          -> bentryEndAddr block endBlock s
+          -> (forall addr, In addr (getAllPaddrBlock startBlock endBlock)
+              -> ~In addr (getPartitions multiplexer s)
+                  /\ (forall part, In part (getPartitions multiplexer s)
+                      -> ~In addr (filterOptionPaddr (getKSEntries part s))
+                          /\ ~In addr (getConfigPaddr part s))
+                  /\ (isBE addr s -> addr + scoffset < endBlock)
+                  /\ (isKS addr s -> addr + nextoffset < endBlock)
+                  /\ addr <> nullAddr))
     /\ (exists s0, consistency s0
         /\ (forall addr, addr <> blockStartAddr -> lookup addr (memory s) beqAddr = lookup addr (memory s0) beqAddr)
         (*TODO will probably need to add more links between s and s0*)
@@ -1455,16 +4142,6 @@ intro eraseSucc. eapply bindRev.
   intuition. exists s0. unfold consistency; unfold consistency1; unfold consistency2; intuition.
 }
 intro currKernelStructureStart. eapply bindRev.
-{ (** MAL.readBlockStartFromBlockEntryAddr **)
-  eapply weaken. apply readBlockStartFromBlockEntryAddr. intros s Hprops. split. apply Hprops.
-  destruct Hprops as ((Heq & Hres & _) & _). subst. assumption.
-}
-intro globalIdPDChildToDelete. eapply bindRev.
-{ (** MAL.readBlockEndFromBlockEntryAddr **)
-  eapply weaken. apply readBlockEndFromBlockEntryAddr. intros s Hprops. split. apply Hprops.
-  destruct Hprops as (((Heq & Hres & _) & _) & _). subst. assumption.
-}
-intro endPDChildToDelete. eapply bindRev.
 { (** Internal.deleteSharedBlocksRec **)
   eapply weaken. (*TODO HERE*) apply deleteSharedBlocksRec. intros s Hprops.
   
